theories/L6_PCPS/lambda_lifting_correct.v
@@ -17,9 +17,9 @@ Section Lambda_lifting_correct.
   Variable cenv : cEnv.
 
   (** The invariant that relates the original function definitions with the lifted ones *)
-  Definition Funs_inv k (rho rho' : env) σ (m : var -> option (var * fTag * list var)) :=
+  Definition Funs_inv k (rho rho' : env) (σ : var -> var) (ζ : var -> option (var * fTag * list var)) :=
     forall f f' ft' fvs vs1 vs2 j ft1  rho1 rho1' B1 f1 xs1 e1,
-      m f = Some (f', ft', fvs) ->
+      ζ f = Some (f', ft', fvs) ->
       M.get f rho = Some (Vfun rho1 B1 f1) ->
       length vs1 = length vs2 ->
       find_def f1 B1 = Some (ft1, xs1, e1) ->
@@ -32,21 +32,15 @@ Section Lambda_lifting_correct.
         (j < k -> Forall2 (preord_val pr cenv j) vs1 vs2 ->
          preord_exp pr cenv j (e1, rho1') (e2, rho2')).
 
-  (* Maps from the original name to the name of the lifted function *)
+  (*& Map from the original name to the name of the lifted function *)
   Definition lifted_name (ζ : var -> option (var * fTag * list var)) : var -> option var :=
     fun f => (liftM (fun x => (fst (fst x)))) (ζ f).
-  
-  Definition domain {A B} (f : A -> option B) : Ensemble A :=
-    fun x => exists y, f x = Some y.
-
-  Definition image' {A B} (f : A -> option B) S : Ensemble B :=
-    fun y => exists x, In _ S x /\ f x = Some y.
   
   (** The domain of ζ *)
   Definition Funs (ζ : var -> option (var * fTag * list var)) : Ensemble var :=
     domain (lifted_name ζ).
   
-  (** The image of ζ on its domain *)
+  (** The image of ζ on its domain - i.e. the names of the lifted functions *)
   Definition LiftedFuns (ζ : var -> option (var * fTag * list var)) : Ensemble var :=
     image' (lifted_name ζ) (Funs ζ).
 
@@ -59,7 +53,7 @@ Section Lambda_lifting_correct.
   Definition FunsFVsLst (ζ : var -> option (var * fTag * list var)) : Ensemble (list var) :=
     fun fvs => exists f f' ft', ζ f = Some (f', ft', fvs).
   
-  (** * [lifted_name] lemmas *)
+  (** * Lemmas about [lifted_name], [Funs], [LiftedFuns], [FunsFVs] and [FunsFVsLst] *)
 
   Lemma lifted_name_extend f x x' xs l :
     f_eq (lifted_name (f {x ~> Some (x', xs, l)})) ((lifted_name f) { x ~> Some x' }).
@@ -77,66 +71,59 @@ Section Lambda_lifting_correct.
     intros Heq; unfold lifted_name; rewrite Heq; eauto.
   Qed.
 
+  Lemma Funs_extend_Some ζ f f' ft fvs :
+    Included _ (Funs (ζ {f ~> Some (f', ft, fvs)}))
+             (Union _ (Funs ζ) (Singleton _ f)).
+  Proof.
+    intros x [val H].
+    destruct (peq f x); subst.
+    - rewrite lifted_name_extend, extend_gss in H. inv H. eauto.
+    - rewrite lifted_name_extend, extend_gso in H; eauto.
+      left. eexists; eauto.
+  Qed.
+
+  Lemma LiftedFuns_extend_Some ζ f f' ft fvs :
+    Included _ (LiftedFuns (ζ {f ~> Some (f', ft, fvs)}))
+            (Union _ (LiftedFuns ζ) (Singleton _ f')).
+  Proof.
+    intros x [g [H1 H2]].
+    destruct (peq f g); subst; rewrite lifted_name_extend in H2;
+    apply Funs_extend_Some in H1.
+    - rewrite extend_gss in H2. inv H2. eauto.
+    - rewrite extend_gso in H2; eauto. inv H1; eauto.
+      left. repeat eexists; eauto.
+      inv H; congruence.
+  Qed.
   
-  Lemma Forall2_preord_var_env_map k P σ rho rho' l :
-    preord_env_P_inj pr cenv P k σ rho rho' ->
-    Included _ (FromList l) P ->
-    Forall2 (preord_var_env pr cenv k rho rho') l (map σ l).
-  Proof with now eauto with Ensembles_DB.
-    induction l; intros Henv Hin; simpl; constructor.
-    - eapply Henv. eapply Hin. rewrite FromList_cons...
-    - eapply IHl; eauto.
-      eapply Included_trans; [| eassumption ].
-      rewrite FromList_cons...
+  Lemma FunsFVs_extend_Some ζ f f' ft fvs :
+    Included _ (FunsFVs (ζ {f ~> Some (f', ft, fvs)}))
+            (Union _ (FunsFVs ζ) (FromList fvs)).
+  Proof.
+    intros x [g [g' [gt' [fvs' [H1 H2]]]]].
+    destruct (peq f g); subst.
+    - rewrite extend_gss in H1. inv H1. eauto.
+    - rewrite extend_gso in H1; eauto.
+      left. eexists; eauto.
+  Qed.
+  
+  Lemma FunsFVs_extend_Some_eq ζ f f' ft fvs :
+    ~ In _ (Funs ζ) f ->
+    Same_set var (FunsFVs (ζ {f ~> Some (f', ft, fvs)}))
+             (Union var (FunsFVs ζ) (FromList fvs)).
+  Proof.
+    intros Hn; split.
+    - now apply FunsFVs_extend_Some.
+    - intros x Hin. inv Hin.
+      destruct H as [g [g' [fg [l [Heq Hin]]]]].
+      repeat eexists; eauto. rewrite extend_gso.
+      eassumption. intros Hc; apply Hn. subst.
+      repeat eexists; eauto. eapply lifted_name_eq.
+      subst. eassumption.
+      repeat eexists; eauto. rewrite extend_gss.
+      reflexivity.
   Qed.
 
-  Lemma image_extend_Included' {A} f x x' S :
-    Included A (image (f {x ~> x'}) S)
-             (Union A (image f (Setminus _ S (Singleton _ x))) (Singleton A x')).
-  Proof.
-    intros y [y' [Hin Heq]]; subst.
-    destruct (peq x y'); subst.
-    - rewrite extend_gss. eauto.
-    - left. rewrite extend_gso; eauto.
-      eexists. split; eauto.
-      constructor; eauto. intros Hc; inv Hc; congruence.
-  Qed.
-
-  Lemma map_extend_not_In {A} f l x (x' : A) :
-    ~ In _ (FromList l) x ->
-    map (f{x~>x'}) l = map f l.
-  Proof.
-    induction l; intros Hnin; eauto.
-    simpl. rewrite extend_gso.
-    f_equal. eapply IHl.
-    intros Hc; eapply Hnin; rewrite FromList_cons; eauto.
-    intros Hc; eapply Hnin; subst; rewrite FromList_cons; eauto.
-  Qed.
-
-  Lemma map_extend_lst_Disjoint {A} f l xs (xs' : list A) :
-    Disjoint _ (FromList l) (FromList xs)  ->
-    map (f <{xs ~> xs'}> ) l = map f l.
-  Proof.
-    revert xs'; induction xs; intros xs' HD; eauto.
-    destruct xs'; eauto. simpl.
-    rewrite FromList_cons in HD.
-    rewrite map_extend_not_In. eapply IHxs.
-    now eauto with Ensembles_DB.
-    intros Hc. eapply HD; eauto.
-  Qed.
-
-  Lemma map_extend_lst_same {A} f xs (xs' : list A) :
-    NoDup xs ->
-    length xs = length xs' ->
-    map (f <{xs ~> xs'}> ) xs = xs'.
-  Proof.
-    revert xs'; induction xs; intros xs' Hnd Hlen; eauto.
-    - destruct xs'; try discriminate. reflexivity.
-    - simpl. destruct xs'; try discriminate.
-      inv Hnd. inv Hlen.
-      rewrite extend_gss. f_equal.
-      rewrite map_extend_not_In; eauto.
-  Qed.
+  (** * Lemmas about [Funs_inv] *)  
   
   Lemma Funs_inv_set k rho rho' σ ζ v1 v2 x y :
     ~ In _ (Funs ζ) x ->
@@ -167,56 +154,6 @@ Section Lambda_lifting_correct.
       rewrite extend_gso in Heq'; eauto. eapply Hnin4.
       repeat eexists; eassumption.
   Qed.
-  
-  Lemma getlist_setlist {A} xs (vs : list A) rho rho' :
-    NoDup xs ->
-    setlist xs vs rho = Some rho' ->
-    getlist xs rho' = Some vs.
-  Proof.
-    revert rho' vs; induction xs; intros rho' vs Hnd Hset.
-    - inv Hset. destruct vs; try discriminate. reflexivity.
-    - inv Hnd. simpl in *.
-      destruct vs; try discriminate.
-      destruct (setlist xs vs rho) eqn:Hset'; try discriminate. inv Hset.
-      rewrite M.gss. rewrite getlist_set_neq.
-      now erewrite IHxs; eauto. eassumption.
-  Qed.
-
-  Lemma getlist_setlist_Disjoint {A} xs xs' (vs : list A) rho rho' :
-    Disjoint _ (FromList xs) (FromList xs') ->
-    setlist xs vs rho = Some rho' ->
-    getlist xs' rho' = getlist xs' rho.
-  Proof with now eauto with Ensembles_DB.
-    revert rho' vs; induction xs; intros rho' vs Hd Hset.
-    - inv Hset. destruct vs; try discriminate. inv H0; reflexivity.
-    - simpl in *.
-      destruct vs; try discriminate.
-      destruct (setlist xs vs rho) eqn:Hset'; try discriminate. inv Hset.
-      rewrite FromList_cons in Hd.
-      rewrite getlist_set_neq.
-      erewrite IHxs...
-      intros Hc; eapply Hd. constructor; eauto.
-  Qed.
-
-  Lemma getlist_def_funs_Disjoint xs B B' rho  :
-    Disjoint _ (FromList xs) (name_in_fundefs B) ->
-    getlist xs (def_funs B' B rho rho) = getlist xs rho.
-  Proof with now eauto with Ensembles_DB.
-    induction B; intros Hd.
-    - simpl.
-      rewrite getlist_set_neq.
-      erewrite IHB...
-      intros Hc; eapply Hd. constructor; eauto. now left.
-    - reflexivity.
-  Qed.
-
-  Instance map_proper {A B} : Proper (f_eq ==> eq ==> eq) (@map A B).
-  Proof.
-    intros f1 f2 Hfeq x1 x2 Heq; subst.
-    induction x2; eauto.
-    simpl. rewrite Hfeq. congruence.
-  Qed.
-
 
   Lemma Funs_inv_setlist k rho rho' rho1 rho1' σ ζ vs1 vs2 xs ys :
     setlist xs vs1 rho = Some rho1 ->
@@ -256,224 +193,6 @@ Section Lambda_lifting_correct.
       repeat eexists; eassumption.
   Qed.
 
-  (* Lemma Funs_inv_setlist_r k rho rho' rho'' σ ζ vs  xs ys : *)
-  (*   setlist ys vs rho' = Some rho'' ->                          *)
-  (*   Funs_inv k rho rho' σ ζ -> *)
-  (*   Disjoint _ (LiftedFuns ζ) (FromList ys) -> *)
-  (*   Disjoint _ (FunsFVs ζ) (FromList xs) -> *)
-  (*   Disjoint _ (image σ (Setminus _ (FunsFVs ζ) (FromList xs))) (FromList ys) -> *)
-  (*   Funs_inv k rho rho'' (σ <{xs ~> ys}>) ζ. *)
-  (* Proof. *)
-  (*   intros Hset1 Hinv HD2 HD3 HD4 f f' ft' fvs vs1' vs2' j ft1  rho2 rho2' B1 f1 *)
-  (*          xs1 e1 Hget1 Hget2 Hlen Hdef Hset. *)
-  (*   edestruct Hinv as *)
-  (*       [rho3 [rho3' [B2 [f2 [xs2 [e2 [vs2'' [Hget' [Hdef' [Hgetl [Hset' Hpre]]]]]]]]]]]; eauto. *)
-  (*   do 8 eexists; repeat split; eauto. *)
-  (*   - erewrite <- setlist_not_In; eauto. *)
-  (*     intros Hc; subst. eapply HD2. constructor; eauto. eexists; eauto. *)
-  (*   - erewrite getlist_setlist_Disjoint; eauto. *)
-  (*     rewrite map_extend_lst_Disjoint. eassumption. *)
-  (*     eapply Disjoint_Included_l; [| eassumption ]. *)
-  (*     repeat eexists; eassumption. *)
-  (*     eapply Disjoint_Included_r_sym; [| eassumption ]. *)
-  (*     rewrite map_extend_lst_Disjoint. *)
-  (*     intros x Hin. unfold In, FromList in Hin. eapply list_in_map_inv in Hin. *)
-  (*     edestruct Hin as [x' [Heq Hin']]. eexists; split; eauto. *)
-  (*     constructor.  *)
-  (*     repeat eexists; eassumption. *)
-  (*     intros Hc. eapply HD3. constructor; eauto. *)
-  (*     repeat eexists; eauto. *)
-  (*     eapply Disjoint_Included_l; [| eassumption ]. *)
-  (*     repeat eexists; eassumption. *)
-  (* Qed. *)
-
-  Lemma getlist_reset {A} σ x y (v : A) rho l :
-    M.get (σ x) rho = Some v ->
-    ~ In _ (image σ (Setminus _ (FromList l) (Singleton _ x))) y ->
-    getlist (map σ l) rho = getlist (map (σ { x ~> y }) l) (M.set y v rho).
-  Proof with now eauto with Ensembles_DB.
-    intros Hget Hnin. induction l; eauto.
-    simpl. destruct (peq x a); subst.
-    - rewrite extend_gss, M.gss, Hget.
-      rewrite IHl. reflexivity.
-      intros Hc. eapply Hnin.
-      rewrite FromList_cons.
-      eapply image_monotonic; try eassumption...      
-    - rewrite extend_gso; eauto.
-      rewrite M.gso.
-      rewrite IHl. reflexivity.
-      intros Hc. eapply Hnin.
-      rewrite FromList_cons.
-      eapply image_monotonic; try eassumption...
-      intros Hc. eapply Hnin.
-      subst. rewrite FromList_cons. eexists; split; eauto.
-      constructor; eauto.
-      intros Hc; inv Hc. congruence.
-  Qed.
-  
-  Lemma getlist_reset_neq {A} σ x y (v : A) rho l :
-    ~ In _ (image σ (Setminus _ (FromList l) (Singleton _ x))) y ->
-    ~ List.In x l -> 
-    getlist (map σ l) rho = getlist (map (σ { x ~> y }) l) (M.set y v rho).
-  Proof with now eauto with Ensembles_DB.
-    intros  Hnin. induction l; intros Hnin'; eauto.
-    simpl. destruct (peq x a); subst.
-    - exfalso. eapply Hnin'. now constructor.
-    - rewrite extend_gso; eauto.
-      rewrite M.gso.
-      rewrite IHl. reflexivity.
-      intros Hc. eapply Hnin.
-      rewrite FromList_cons.
-      eapply image_monotonic; try eassumption...
-      intros Hc. eapply Hnin'. now constructor 2.
-      intros Hc. subst. eapply Hnin.
-      rewrite FromList_cons. eexists; split; eauto.
-      constructor; eauto.
-      intros Hc; inv Hc. congruence.
-  Qed.
-
-  Lemma image_extend_lst_Included {A} f S xs xs' :
-    length xs = length xs' ->
-    Included _ (image (f <{xs ~> xs'}>) S) (Union A (image f (Setminus _ S (FromList xs))) (FromList xs')).
-  Proof with now eauto with Ensembles_DB.
-    revert xs' f S; induction xs; intros xs' f S Hlen.
-    - simpl. rewrite FromList_nil, Setminus_Empty_set_neut_r...
-    - destruct xs'; try discriminate. inv Hlen.
-      simpl. eapply Included_trans.
-      apply image_extend_Included'. rewrite !FromList_cons.
-      eapply Union_Included; [| now eauto with Ensembles_DB ].
-      eapply Included_trans. eapply IHxs; eauto.
-      apply Included_Union_compat.
-      eapply image_monotonic...
-      now eauto with Ensembles_DB.
-  Qed.
-  
-  Lemma extend_commut {A} f y x x' (y' : A) :
-    x' <> x -> y' <> y ->
-    f_eq ((f {x ~> y}) {x' ~> y'}) ((f {x' ~> y'}) {x ~> y}).
-  Proof.
-    intros Hnin Hnin' z.
-    destruct (peq x z); subst.
-    - rewrite extend_gss, extend_gso; eauto.
-      now rewrite extend_gss.
-    - destruct (peq x' z); subst.
-      + rewrite extend_gss, (extend_gso _ x y z); eauto.
-        now rewrite extend_gss.
-      + repeat rewrite extend_gso; eauto.
-  Qed.
-        
-  Lemma extend_extend_lst_commut {A} f ys xs x (y : A) :
-    ~ List.In x xs ->
-    ~ List.In y ys ->
-    length xs = length ys ->
-    f_eq ((f {x ~> y}) <{xs ~> ys}>) ((f <{xs ~> ys}>) {x ~> y}).
-  Proof.
-    revert f ys; induction xs; intros f ys Hnin1 Hnin2 Hlen; simpl.
-    - reflexivity.
-    - destruct ys; try discriminate. inv Hlen.
-      rewrite IHxs. rewrite extend_commut. reflexivity.
-      intros Hc; subst. now eapply Hnin1; constructor.
-      intros Hc; subst. now eapply Hnin2; constructor.
-      intros Hc; subst. now eapply Hnin1; constructor 2.
-      intros Hc; subst. now eapply Hnin2; constructor 2.
-      eassumption.
-  Qed.
-
-  Lemma set_permut {A} rho x y (v1 v2 : A) z :
-    x <> y ->
-    M.get z (M.set x v1 (M.set y v2 rho)) =
-    M.get z (M.set y v2 (M.set x v1 rho)).
-  Proof.
-    intros Hnin. destruct (peq z x); subst.
-    - rewrite M.gss, M.gso, M.gss; eauto.
-    - rewrite (@M.gso _ z x); eauto.
-      destruct (peq z y); subst.
-      + rewrite !M.gss; eauto.
-      + rewrite !M.gso; eauto.
-  Qed.
-
-  Lemma set_setlist_permut {A} rho rho' y ys (v : A) vs :
-    setlist ys vs rho = Some rho' ->
-    ~ List.In y ys ->
-    exists rho'',
-      setlist ys vs (M.set y v rho) = Some rho'' /\
-      (forall z, M.get z (M.set y v rho') = M.get z rho'').
-  Proof.
-    revert vs rho'.
-    induction ys; intros vs rho' Hset Hin;
-    destruct vs; try discriminate.
-    - inv Hset. eexists; split; simpl; eauto.
-    - simpl in Hset.
-      destruct (setlist ys vs rho) eqn:Heq; try discriminate.
-      inv Hset. edestruct IHys as [rho'' [Hset Hget]]; eauto.
-      intros Hc; eapply Hin; now constructor 2.
-      eexists; split.
-      simpl. rewrite Hset. reflexivity.
-      intros z. rewrite set_permut.
-      destruct (peq z a); subst.
-      + rewrite !M.gss; eauto.
-      + rewrite !(@M.gso _ z a); eauto.
-      + intros Hc. eapply Hin.
-        constructor; eauto.
-  Qed.
-  
-  Lemma get_eq_getlist_eq {A} (rho rho' : M.t A) xs :
-    (forall z, M.get z rho = M.get z rho') ->
-    getlist xs rho = getlist xs rho'.
-  Proof.
-    induction xs; intros H; eauto.
-    simpl; f_equal.
-    rewrite IHxs; eauto.
-    rewrite H. reflexivity.
-  Qed.
-
-  Lemma getlist_reset_lst σ xs ys (vs : list val) rho rho' l  : 
-    setlist ys vs rho = Some rho' ->
-    getlist (map σ xs) rho = Some vs ->
-    Disjoint _ (image σ (FromList l)) (FromList ys) ->
-    length xs = length ys ->
-    NoDup xs -> NoDup ys ->
-    getlist (map σ l) rho = getlist (map (σ <{ xs ~> ys }>) l) rho'.
-  Proof with now eauto with Ensembles_DB.
-    revert σ ys vs rho' rho. induction xs as [| x xs IHxs ];
-      intros σ ys vs rho' rho Hset Hget HD Hlen Hnd1 Hnd2.
-    - destruct ys; try discriminate.
-      inv Hget. inv Hset. reflexivity.
-    - destruct ys; try discriminate. simpl in *.
-      inv Hlen. destruct vs; try discriminate.
-      destruct (setlist ys vs rho) eqn:Hset'; try discriminate.
-      destruct (M.get (σ x) rho) eqn:Hget'; try discriminate.
-      destruct (getlist (map σ xs) rho) eqn:Hgetl; try discriminate.
-      inv Hget. inv Hset. inv Hnd1. inv Hnd2. rewrite !FromList_cons in HD.
-      assert (H : getlist (map ((σ <{ xs ~> ys }>) {x ~> e}) l) (M.set e v t) =
-                  getlist (map ((σ <{ xs ~> ys }>)) l) t).
-      { destruct (in_dec peq x l).
-        - rewrite <- getlist_reset; try reflexivity.
-          rewrite extend_lst_gso; eauto.
-          erewrite <- setlist_not_In. eassumption. eassumption.
-          intros Hc. eapply HD. constructor; eauto.
-          eexists; split; eauto. 
-          intros Hc.
-          apply image_extend_lst_Included in Hc; eauto.
-          inv Hc; eauto. eapply HD. constructor; eauto.
-          eapply image_monotonic; [| eassumption ]...
-        - rewrite map_extend_not_In; eauto.
-          erewrite getlist_set_neq. reflexivity.
-          intros Hc. eapply in_map_iff in Hc.
-          destruct Hc as [x' [Heq Hin]]. 
-          destruct (in_dec peq x' xs).
-          + edestruct (extend_lst_gss σ) as [y' [Hin' Heq']]; eauto.
-            rewrite Heq in Hin'. subst.
-            subst. eauto.
-          + rewrite extend_lst_gso in Heq; eauto.
-            eapply HD. constructor; eauto.
-            eexists; eauto. }
-      rewrite H.
-      erewrite <- IHxs; eauto.
-      now eauto with Ensembles_DB.
-  Qed.
-
-
   Lemma Funs_inv_setlist_getlist_r k rho rho' rho'' σ ζ vs xs ys :
     setlist ys vs rho' = Some rho'' ->
     getlist (map σ xs) rho' = Some vs ->
@@ -499,278 +218,7 @@ Section Lambda_lifting_correct.
       eapply image_monotonic. 
       intros x Hin. repeat eexists; eauto.
   Qed.
-  
-  Lemma preord_env_P_inj_getlist_l (P : var -> Prop) k f rho1 rho2 xs vs1 :
-    preord_env_P_inj pr cenv P k f rho1 rho2 ->
-    Included var (FromList xs) P ->
-    getlist xs rho1 = Some vs1 ->
-    exists vs2 : list val,
-      getlist (map f xs) rho2 = Some vs2 /\ Forall2 (preord_val pr cenv k) vs1 vs2.
-  Proof with now eauto with Ensembles_DB.
-    revert vs1. induction xs; intros vs1 Henv Hinc Hget.
-    - eexists; split; eauto. inv Hget. constructor.
-    - simpl in *.
-      destruct (M.get a rho1) eqn:Hgeta; try discriminate.
-      destruct (getlist xs rho1) eqn:Hgetl; try discriminate.
-      inv Hget.
-      edestruct Henv with (x := a) as [x' [Hgetx' Hprex']]. eapply Hinc. rewrite FromList_cons...
-      eassumption.
-      edestruct IHxs as [l' [Hgetl' Hprel']]. eassumption.
-      eapply Included_trans; [| eassumption ]. rewrite FromList_cons...
-      reflexivity.
-      eexists. rewrite Hgetx', Hgetl'. split.
-      reflexivity.
-      now constructor; eauto.
-  Qed.
 
-  Lemma getlist_app {A} m l1 l2 (v1 v2 : list A) :
-    getlist l1 m = Some v1 ->
-    getlist l2 m = Some v2 ->
-    getlist (l1 ++ l2) m = Some (v1 ++ v2).
-  Proof.
-    revert v1. induction l1; intros v1 Hget1 Hget2; simpl in *.
-    - inv Hget1. eauto.
-    - destruct (M.get a m) eqn:Hgeta; try discriminate.
-      destruct (getlist l1 m) eqn:Hget; try discriminate.
-      inv Hget1. simpl. erewrite IHl1; eauto.
-  Qed.
-
-  Lemma preord_env_P_inj_set_not_In_P_l P k f rho1 rho2 x v :
-    preord_env_P_inj pr cenv P k f rho1 rho2 ->
-    ~ In _ P x ->
-    preord_env_P_inj pr cenv P k f (M.set x v rho1) rho2.
-  Proof.
-    intros Henv Hnin y Hy v' Hget. eapply Henv. eassumption.
-    rewrite M.gso in Hget. eassumption. intros Hc; subst.
-    eauto.
-  Qed.
-
-  Lemma preord_env_P_inj_set_not_In_P_r P k f rho1 rho2 x v :
-    preord_env_P_inj pr cenv P k f rho1 rho2 ->
-    ~ In _ (image f P) x ->    
-    preord_env_P_inj pr cenv P k f rho1 (M.set x v rho2).
-  Proof.
-    intros Henv Hnin y Hy v' Hget.
-    edestruct Henv as [v'' [Hget' Hv]]; eauto.
-    eexists; split; eauto.
-    rewrite M.gso. eassumption. intros Hc; subst.
-    eapply Hnin. eexists; eauto.
-  Qed.
-
-  Lemma Add_functions_free_set_Included B fvs ζ σ S ζ' σ' S' :
-    Add_functions B fvs ζ σ S ζ' σ' S' ->
-    Included _ S' S.
-  Proof with now eauto with Ensembles_DB.
-    intros Hadd. induction Hadd...
-  Qed.
-
-  Lemma Lambda_lift_free_set_Included_mut :
-    (forall e ζ σ S e' S',
-       Exp_lambda_lift ζ σ e S e' S' ->
-       Included _ S' S) /\
-    (forall B ζ σ S B' S',
-       Fundefs_lambda_lift ζ σ B S B' S' ->
-       Included _ S' S).
-  Proof with now eauto with Ensembles_DB.
-    exp_defs_induction IHe IHl IHB; intros; inv H; try now eauto with Ensembles_DB.
-    - eapply Included_trans. now eapply IHl; eauto.
-      eapply IHe; eauto.
-    - eapply Included_trans. now eapply IHe; eauto.
-      eapply Included_trans. now eapply IHB; eauto.
-      eapply Add_functions_free_set_Included; eauto.
-    - eapply Included_trans. now eapply IHB; eauto.
-      eapply Included_trans. now eapply IHe; eauto.
-      now eauto with Ensembles_DB.
-  Qed.
-
-  Corollary Exp_Lambda_lift_free_set_Included :
-    forall e ζ σ S e' S',
-      Exp_lambda_lift ζ σ e S e' S' ->
-      Included _ S' S.
-  Proof.
-    destruct Lambda_lift_free_set_Included_mut; eauto.
-  Qed.
-
-  Corollary Fundefs_Lambda_lift_free_set_Included :
-    forall B ζ σ S B' S',
-      Fundefs_lambda_lift ζ σ B S B' S' ->
-      Included _ S' S.
-  Proof.
-    destruct Lambda_lift_free_set_Included_mut; eauto.
-  Qed.
-  
-  Lemma Fundefs_lambda_lift_find_def σ ζ S1 B1 S2 B2 f t xs1 e1 f' t' fvs :
-    Fundefs_lambda_lift ζ σ B1 S1 B2 S2 ->
-    ζ f = Some (f', t', fvs) ->
-    Disjoint _ (bound_var_fundefs B1) (LiftedFuns ζ) ->
-    injective_subdomain (name_in_fundefs B1) (lifted_name ζ) ->
-    find_def f B1 = Some (t, xs1, e1) ->
-    exists (xs1' ys : list var) (e2 : exp) S2 S2',
-      find_def f B2 = Some (t, xs1', (Eapp f' t' (xs1' ++ map σ fvs))) /\
-      find_def f' B2 = Some (t', xs1 ++ ys, e2) /\
-      NoDup ys /\ NoDup xs1' /\
-      length xs1 = length xs1' /\
-      length ys = length fvs /\
-      Included _ S2 S1 /\
-      Included _ (FromList ys) S1 /\
-      Included _ (FromList xs1') S1 /\
-      Disjoint _ (FromList ys) S2 /\
-      Disjoint _ (FromList xs1') S2 /\
-      Disjoint _ (FromList xs1') (FromList ys) /\
-      Exp_lambda_lift ζ (σ <{ xs1 ++ fvs ~> xs1 ++ ys }>) e1 S2 e2 S2'.
-  Proof with now eauto with Ensembles_DB.
-    intros Hll. induction Hll; intros Heq HD Hinj Hdef.
-    - assert (Heq' := lifted_name_eq _ _ _ _ _ Heq).
-      simpl in Hdef. destruct (M.elt_eq f f0); subst.
-      + rewrite Heq in H; inv H. inv Hdef.
-        exists xs', ys, e'. do 2 eexists.
-        split; [| split; [| split; [| split; [| split; [| split; [| split; [| split; [| split; [| split; [| split; [| split]]]]]]]]]]];
-        [ | | | | | | | | | | | | eassumption ]; eauto.
-        * simpl. rewrite peq_false, peq_true. reflexivity.
-          intros Hc. subst. eapply HD. constructor; eauto.
-          repeat eexists; eauto.
-        * simpl. rewrite peq_true. reflexivity.
-        * now eauto with Ensembles_DB.
-        * eapply Included_trans; [ eassumption |]...
-        * now eauto with Ensembles_DB.
-        * now eauto with Ensembles_DB.
-        * eapply Disjoint_Included_l; [ eassumption |]...
-      + destruct IHHll as (xs1' & ys' & e2 & S2 & S2' & Hf1 & Hf2 & Hnd1 & Hnd2
-                                & Heq1 & Heq2 & Hinc1 & Hinc2 & Hinc3 & Hd1 & Hd2 & Hd3 & Hexp).
-        eassumption. normalize_bound_var_in_ctx...
-        eapply injective_subdomain_antimon. eassumption.
-        now eauto with Ensembles_DB. eassumption.
-        eexists xs1', ys', e2. do 2 eexists.
-        split; [| split; [| split; [| split; [| split; [| split; [| split; [| split; [| split; [| split; [| split; [| split]]]]]]]]]]];
-        [ | | | | | | | | | | | | eassumption ]; eauto.
-        * simpl. rewrite peq_false; eauto. rewrite peq_false; now eauto.
-          intros Hc. subst. eapply HD. constructor.
-          constructor 2. apply name_in_fundefs_bound_var_fundefs.
-          eapply fun_in_fundefs_name_in_fundefs. eapply find_def_correct.
-          eassumption. eexists.
-          split; repeat eexists; now unfold lifted_name; rewrite H; eauto.
-        * simpl. rewrite peq_false; eauto. rewrite peq_false; eauto.
-          intros Hc. subst. eapply HD. constructor. now eauto.
-          now repeat eexists; eauto.
-          intros Hc; subst. eapply n. eapply Hinj.
-          constructor 2. eapply fun_in_fundefs_name_in_fundefs.
-          eapply find_def_correct. eassumption.
-          now simpl; eauto. erewrite !lifted_name_eq; eauto.
-        * eapply Included_trans. eassumption.
-          eapply Included_trans. eapply Exp_Lambda_lift_free_set_Included.
-          eassumption.
-          now eauto with Ensembles_DB.
-        * eapply Included_trans. eassumption.
-          eapply Included_trans.
-          eapply Exp_Lambda_lift_free_set_Included; now eauto.
-          now eauto with Ensembles_DB.
-        * eapply Included_trans. eassumption.
-          eapply Included_trans.
-          eapply Exp_Lambda_lift_free_set_Included; now eauto.
-          now eauto with Ensembles_DB.
-    - inv Hdef.
-  Qed.
-  
-
-  Lemma setlist_app {A} xs1 xs2 (vs1 vs2 : list A) rho rho' : 
-    setlist (xs1 ++ xs2) (vs1 ++ vs2) rho = Some rho' ->
-    length xs1 = length vs1 ->
-    exists rho'',
-      setlist xs2 vs2 rho = Some rho'' /\
-      setlist xs1 vs1 rho'' = Some rho'.
-  Proof.
-    revert vs1 rho'. induction xs1; intros vs1 rho' Hset Hlen.
-    - destruct vs1; try discriminate.
-      eexists; split; eauto.
-    - destruct vs1; try discriminate.
-      inv Hlen. simpl in Hset.
-      destruct (setlist (xs1 ++ xs2) (vs1 ++ vs2) rho) eqn:Heq; try discriminate.
-      inv Hset. edestruct IHxs1 as [rho'' [Hset1 Hset2]].
-      eassumption. eassumption.
-      eexists. split. eassumption. simpl; rewrite Hset2; reflexivity.
-  Qed.
-
-  Lemma extend_lst_app {A} (f : positive -> A) xs xs' ys ys' :
-    length xs = length ys -> 
-    f_eq (f <{xs ++ xs' ~> ys ++ ys'}>)
-         (f <{xs' ~> ys'}> <{xs ~> ys}>).
-  Proof.
-    revert ys f. induction xs; intros ys f Hlen.
-    - simpl. destruct ys; try discriminate. reflexivity.
-    - destruct ys; try discriminate. simpl.
-      eapply f_eq_extend.
-      eapply IHxs. inv Hlen. reflexivity.
-  Qed.
-
-  Instance preord_env_P_inj_f_proper : Proper (eq ==> eq ==> f_eq ==> eq ==> eq ==> iff)
-                                              (preord_env_P_inj pr cenv).
-  Proof.
-    constructor; subst; intros Hp.
-    intros z Hz. rewrite <- H1. eauto.
-    intros z Hz. rewrite H1. eauto.
-  Qed.  
-  
-  Lemma preord_env_P_inj_reset P k f rho rho' x y v :
-    M.get (f x) rho' = Some v ->
-    ~ In _ (image f P) y ->
-    preord_env_P_inj pr cenv P k f rho rho' ->
-    preord_env_P_inj pr cenv P k (f {x ~> y}) rho (M.set y v rho').
-  Proof.
-    intros Hget Hnin Hpre z Hz v' Hget'.
-    destruct (peq z x); subst.
-    - rewrite extend_gss, M.gss.
-      edestruct Hpre as [v2 [Hget'' Hpre2]]; eauto.
-      rewrite Hget'' in Hget; inv Hget.
-      eexists; eauto.
-    - rewrite extend_gso, M.gso; eauto.
-      eapply Hpre; eauto.
-      intros Hc; subst. eapply Hnin; eexists; eauto.
-  Qed.
-
-
-  Lemma preord_env_P_inj_resetlist P k f rho rho' rho'' xs ys vs :
-    getlist (map f xs) rho' = Some vs ->
-    Disjoint _ (image f P) (FromList ys) ->
-    setlist ys vs rho' = Some rho'' ->
-    NoDup ys ->
-    length xs = length ys ->
-    preord_env_P_inj pr cenv P k f rho rho' ->
-    preord_env_P_inj pr cenv P k (f <{xs ~> ys}>) rho rho''.
-  Proof.
-    revert rho'' ys vs; induction xs; intros rho'' ys vs Hget HD Hset Hdup Hlen Hpre.
-    - simpl. destruct vs; try discriminate.
-      destruct ys; try discriminate. inv Hset. eassumption.
-    - simpl in *.
-      destruct (M.get (f a) rho') eqn:Heqa; try discriminate.
-      destruct (getlist (map f xs) rho') eqn:Hgetl; try discriminate.
-      inv Hget.
-      destruct ys; try discriminate. simpl in Hset.
-      destruct (setlist ys l rho') eqn:Hsetl; try discriminate.
-      rewrite FromList_cons in HD. inv Hset.
-      assert (Hpre' : preord_env_P_inj pr cenv P k (f <{ xs ~> ys }>) rho t).
-      { eapply IHxs. reflexivity.
-        now eauto with Ensembles_DB.
-        eassumption. now inv Hdup. now inv Hlen. eassumption. }
-      intros z Hz v' Hget'.
-      destruct (peq z a); subst.
-      + rewrite extend_gss, M.gss.
-        edestruct Hpre as [v2 [Hget'' Hpre2]]; eauto.
-        rewrite Hget'' in Heqa; inv Heqa.
-        eexists; eauto.
-      + rewrite extend_gso, M.gso; eauto.
-        eapply Hpre'; eauto.
-        inv Hdup. intros Hc; subst.
-        edestruct in_dec with (a := z) (l := xs) as [Hin | Hnin ].
-        now apply peq.
-        edestruct (@extend_lst_gss var f xs ys z) as [x' [Heq Hin']].
-        eassumption. now inv Hlen. eapply H1.
-        rewrite <- Heq in Hin'. eassumption.
-        rewrite extend_lst_gso in H1; [| eassumption ].
-        eapply HD. constructor; eauto.
-        eexists; split; eauto. rewrite extend_lst_gso; [| eassumption ].
-        reflexivity.
-  Qed.
-  
   Lemma Funs_inv_monotonic k i rho rho' σ ζ :
     Funs_inv k rho rho' σ ζ ->
     i <= k ->
@@ -793,531 +241,8 @@ Section Lambda_lifting_correct.
     do 7 eexists; repeat split; eauto.
     rewrite <- H2. eassumption.
     rewrite H2. eassumption.
-  Qed.
-
-  Lemma binding_in_map_getlist {A} S m  xs :
-    binding_in_map S m ->
-    Included _  (FromList xs) S ->
-    exists (vs : list A), getlist xs m = Some vs.
-  Proof with now eauto with Ensembles_DB.
-    intros Hin Hinc. induction xs.
-    - eexists; simpl; eauto.
-    - rewrite FromList_cons in Hinc. edestruct Hin with (x := a) as [v' Hget].
-      now eapply Hinc; eauto.
-      edestruct IHxs as [vs' Hgetl].
-      eapply Included_trans...
-      eexists; simpl. rewrite Hget, Hgetl. reflexivity.
-  Qed.
-
-
-  Lemma setlist_length3 rho xs vs : 
-    length xs = length vs ->
-    exists rho' : M.t val, setlist xs vs rho = Some rho'.
-  Proof.
-    revert vs; induction xs; intros vs Hlen; destruct vs; try discriminate.
-    - eexists; simpl; eauto.
-    - inv Hlen.
-      edestruct IHxs as [rho' Hset]. eassumption.
-      eexists. simpl. rewrite Hset. reflexivity.
-  Qed.
-
-  Lemma setlist_length_eq {A} rho rho' xs (vs : list A) :
-    setlist xs vs rho = Some rho' ->
-    length xs = length vs.
-  Proof.
-    revert rho' vs; induction xs; intros rho' vs Hset.
-    - destruct vs; try discriminate. reflexivity.
-    - destruct vs; try discriminate.
-      simpl in Hset.
-      destruct (setlist xs vs rho) eqn:Heq; try discriminate.
-      simpl. f_equal. inv Hset. eauto.
-  Qed.
-
-  Lemma Add_functions_fvs_eq B fvs σ ζ S σ' ζ' S' f f' ft fvs' :
-    Add_functions B fvs σ ζ S σ' ζ' S' ->
-    ζ' f = Some (f', ft, fvs') ->
-    In _ (name_in_fundefs B) f ->
-    fvs' = fvs.
-  Proof.
-    intros Hadd Heq Hin; induction Hadd.
-    - destruct (peq f f0); subst.
-      + rewrite extend_gss in Heq. inv Heq. eauto.
-      + inv Hin. inv H0; congruence.
-        rewrite extend_gso in Heq; eauto.
-    - inv Hin.
-  Qed.
-
-  Lemma injective_subdomain_extend' S f x x' :
-    injective_subdomain (Setminus _ S (Singleton _ x)) f ->
-    ~ In positive (image f (Setminus positive S (Singleton positive x))) x' ->
-    injective_subdomain S (f {x ~> x'}).
-  Proof.
-    intros Hinj Hnin y z Hin Hin' Heq.
-    destruct (peq x y); destruct (peq x z); subst; eauto;
-    try rewrite extend_gss in Heq; try rewrite !extend_gso in Heq; eauto.
-    - subst. exfalso. eapply Hnin. eexists; split; eauto.
-      constructor; eauto.
-      intros Hc; inv Hc; subst; congruence.
-    - subst. exfalso. eapply Hnin. eexists; split; eauto.
-      constructor; eauto.
-      intros Hc; inv Hc; subst; congruence.
-    - subst. eapply Hinj in Heq; eauto.
-      constructor; eauto.
-      intros Hc; inv Hc; subst; congruence.
-      constructor; eauto.
-      intros Hc; inv Hc; subst; congruence.
-  Qed.
-
-
-
-  Lemma injective_subdomain_extend_lst S f xs xs' :
-    injective_subdomain (Setminus _ S (FromList xs)) f ->
-    Disjoint positive (image f (Setminus positive S (FromList xs))) (FromList xs') ->
-    NoDup xs' ->
-    length xs = length xs' ->
-    injective_subdomain S (f <{xs ~> xs'}>).
-  Proof with now eauto with Ensembles_DB.
-    revert xs' f S. induction xs; intros xs' f S Hinj HD Hnd Hlen.
-    - simpl. rewrite FromList_nil, Setminus_Empty_set_neut_r in Hinj. eassumption.
-    - destruct xs'; try discriminate.
-      inv Hlen. simpl.
-      rewrite !FromList_cons in HD. rewrite !FromList_cons in Hinj. inv Hnd.
-      eapply injective_subdomain_extend'.
-      + eapply IHxs. rewrite Setminus_Union. eassumption. 
-        eapply Disjoint_Included; [ | | eassumption ].
-        now eauto with Ensembles_DB.
-        rewrite Setminus_Union. reflexivity.
-        eassumption. eassumption.
-      + intros Hc. eapply image_extend_lst_Included in Hc; eauto.
-        inv Hc.
-        eapply HD. constructor.
-        rewrite <- Setminus_Union. eassumption.
-        now eauto with Ensembles_DB.
-        eapply H2; eassumption.
-  Qed.
-
-  Lemma Add_functions_image_Included P B fvs σ ζ S σ' ζ' S' :
-    Add_functions B fvs σ ζ S σ' ζ' S' ->
-    Included _ (image σ' P) (Union _ (image σ (Setminus _ P (name_in_fundefs B))) (name_in_fundefs B)).
-  Proof with now eauto with Ensembles_DB.
-    intros Hadd. revert P. induction Hadd; intros P.
-    - eapply Included_trans.
-      eapply image_extend_Included'. 
-      eapply Union_Included; [| now eauto with Ensembles_DB ].
-      eapply Included_trans. eapply IHHadd.
-      rewrite Setminus_Union...
-    - now eauto with Ensembles_DB.
-  Qed.
-
-  Instance Proper_domain {A B} : Proper (f_eq ==> Same_set A) (@domain A B).
-  Proof.
-    constructor; intros x' [y' H'].
-    rewrite H in H'. repeat eexists; eauto.
-    rewrite <- H in H'. repeat eexists; eauto.
-  Qed.
-
-  Instance Proper_image' {A B} : Proper (f_eq ==> Same_set _ ==> Same_set B) (@image' A B).
-  Proof.
-    constructor; intros x' [y' [H1 H2]]; inv H0.
-    rewrite H in H2. repeat eexists; eauto.
-    rewrite <- H in H2. repeat eexists; eauto.
-  Qed.
-
-  Lemma Funs_extend_Some ζ f f' ft fvs :
-    Included _ (Funs (ζ {f ~> Some (f', ft, fvs)}))
-            (Union _ (Funs ζ) (Singleton _ f)).
-  Proof.
-    intros x [val H].
-    destruct (peq f x); subst.
-    - rewrite lifted_name_extend, extend_gss in H. inv H. eauto.
-    - rewrite lifted_name_extend, extend_gso in H; eauto.
-      left. eexists; eauto.
-  Qed.
-
-  Lemma LiftedFuns_extend_Some ζ f f' ft fvs :
-    Included _ (LiftedFuns (ζ {f ~> Some (f', ft, fvs)}))
-            (Union _ (LiftedFuns ζ) (Singleton _ f')).
-  Proof.
-    intros x [g [H1 H2]].
-    destruct (peq f g); subst; rewrite lifted_name_extend in H2;
-    apply Funs_extend_Some in H1.
-    - rewrite extend_gss in H2. inv H2. eauto.
-    - rewrite extend_gso in H2; eauto. inv H1; eauto.
-      left. repeat eexists; eauto.
-      inv H; congruence.
-  Qed.
+  Qed.  
   
-  Lemma FunsFVs_extend_Some ζ f f' ft fvs :
-    Included _ (FunsFVs (ζ {f ~> Some (f', ft, fvs)}))
-            (Union _ (FunsFVs ζ) (FromList fvs)).
-  Proof.
-    intros x [g [g' [gt' [fvs' [H1 H2]]]]].
-    destruct (peq f g); subst.
-    - rewrite extend_gss in H1. inv H1. eauto.
-    - rewrite extend_gso in H1; eauto.
-      left. eexists; eauto.
-  Qed.
-  
-  Lemma Add_functions_LiftedFuns_Included B fvs σ ζ S σ' ζ' S' :
-    Add_functions B fvs σ ζ S σ' ζ' S' ->
-    Included _ (LiftedFuns ζ') (Union _ (LiftedFuns ζ) (Setminus _ S S')).
-  Proof with now eauto with Ensembles_DB.
-    intros Hadd. induction Hadd.
-    - eapply Included_trans.
-      eapply LiftedFuns_extend_Some.
-      eapply Union_Included.
-      eapply Included_trans. now eapply IHHadd.
-      now eauto with Ensembles_DB.
-      eapply Included_Union_preserv_r.
-      eapply Singleton_Included. constructor.
-      eapply Add_functions_free_set_Included; eassumption.
-      intros Hc. inv Hc. eauto.
-    - now eauto with Ensembles_DB.
-  Qed.
-
-  Lemma Add_functions_Funs_Included B fvs σ ζ S σ' ζ' S' :
-    Add_functions B fvs σ ζ S σ' ζ' S' ->
-    Included _ (Funs ζ') (Union _ (Funs ζ) (name_in_fundefs B)).
-  Proof with now eauto with Ensembles_DB.
-    intros Hadd. induction Hadd.
-    - eapply Included_trans.
-      eapply Funs_extend_Some.
-      eapply Union_Included.
-      eapply Included_trans. now eapply IHHadd.
-      now eauto with Ensembles_DB.
-      eapply Included_Union_preserv_r...
-    - now eauto with Ensembles_DB.
-  Qed.
-
-  Lemma Add_functions_FunsFVs_Included_r B fvs σ ζ S σ' ζ' S' :
-    Add_functions B fvs σ ζ S σ' ζ' S' ->
-    Included _ (FunsFVs ζ') (Union _ (FunsFVs ζ) (FromList fvs)).
-  Proof with now eauto with Ensembles_DB.
-    intros Hadd. induction Hadd.
-    - eapply Included_trans.
-      eapply FunsFVs_extend_Some.
-      eapply Union_Included.
-      eapply Included_trans. now eapply IHHadd.
-      now eauto with Ensembles_DB.
-      eapply Included_Union_preserv_r...
-    - now eauto with Ensembles_DB.
-  Qed.
-
-  Lemma FunsFVs_extend_Some_eq ζ f f' ft fvs :
-    ~ In _ (Funs ζ) f ->
-    Same_set var (FunsFVs (ζ {f ~> Some (f', ft, fvs)}))
-             (Union var (FunsFVs ζ) (FromList fvs)).
-  Proof.
-    intros Hn; split.
-    - now apply FunsFVs_extend_Some.
-    - intros x Hin. inv Hin.
-      destruct H as [g [g' [fg [l [Heq Hin]]]]].
-      repeat eexists; eauto. rewrite extend_gso.
-      eassumption. intros Hc; apply Hn. subst.
-      repeat eexists; eauto. eapply lifted_name_eq.
-      subst. eassumption.
-      repeat eexists; eauto. rewrite extend_gss.
-      reflexivity.
-  Qed.
-
-  Lemma Add_functions_FunsFVs_Included_l B fvs σ ζ S σ' ζ' S' :
-    Add_functions B fvs σ ζ S σ' ζ' S' ->
-    unique_bindings_fundefs B ->
-    Disjoint _ (Funs ζ) (name_in_fundefs B) ->
-    Included _ (FunsFVs ζ) (FunsFVs ζ').
-  Proof with now eauto with Ensembles_DB.
-    intros Hadd Hun HD. induction Hadd.
-    - inv Hun. eapply Included_trans. eapply IHHadd.
-      eassumption. now eauto with Ensembles_DB.
-      rewrite FunsFVs_extend_Some_eq.
-      now eauto with Ensembles_DB.
-      intros Hc. 
-      eapply Add_functions_Funs_Included in Hc; [| eassumption ].
-      inv Hc. eapply HD. constructor; eauto. left; eauto.
-      eapply H6. apply name_in_fundefs_bound_var_fundefs. eassumption.
-    - now eauto with Ensembles_DB.
-  Qed.
-
-  Lemma f_eq_subdomain_Union {A B} P1 P2 (f1 f2 : A -> B) :
-    f_eq_subdomain P1 f1 f2 ->
-    f_eq_subdomain P2 f1 f2 ->
-    f_eq_subdomain (Union _ P1 P2) f1 f2.
-  Proof.
-    intros H1 H2 x1 HP; inv HP; eauto.
-  Qed.
-    
-  Lemma Add_functions_σ_eq B fvs σ ζ S σ' ζ' S' :
-    Add_functions B fvs σ ζ S σ' ζ' S' ->
-    f_eq_subdomain (Complement _ (name_in_fundefs B)) σ σ'.
-  Proof.
-    intros Hadd. induction Hadd; simpl.
-    - eapply f_eq_subdomain_extend_not_In_S_r.
-      intros Hc; apply Hc. eauto.
-      eapply f_eq_subdomain_antimon; [| eassumption ].
-      now eauto with Ensembles_DB.
-    - reflexivity.
-  Qed.
-
-
-  Lemma Add_functions_lifted_name_Disjoint B fvs σ ζ S σ' ζ' S' :
-    Add_functions B fvs σ ζ S σ' ζ' S' ->
-    unique_bindings_fundefs B ->
-    Disjoint _ (LiftedFuns ζ) S ->
-    Disjoint _ (image (lifted_name ζ') (name_in_fundefs B))
-             (image (lifted_name ζ') (Complement _ (name_in_fundefs B))).
-  Proof.
-    intros Hadd Hun HD. induction Hadd; simpl.
-    - inv Hun. rewrite image_Union. apply Union_Disjoint_l.
-      rewrite image_Singleton.
-      rewrite !lifted_name_extend, !extend_gss.
-      rewrite image_extend_not_In_S; eauto.
-      constructor. intros x Hc. inv Hc. inv H0.
-      destruct H1 as [x' [Hin Heq]].
-      assert (Hin' : In _ (LiftedFuns ζ') f').
-      now repeat eexists; eauto.
-      eapply Add_functions_LiftedFuns_Included in Hin'; [| eassumption ].
-      inv Hin'. eapply HD.  constructor; eauto.
-      eapply Add_functions_free_set_Included; eassumption.
-      inv H0; eauto.
-      eapply Disjoint_Included; [| | now apply IHHadd ].
-      rewrite lifted_name_extend. rewrite image_extend_not_In_S; eauto.
-      apply image_monotonic...
-      now eauto with Ensembles_DB.
-      rewrite lifted_name_extend. rewrite image_extend_not_In_S; eauto.
-      reflexivity. intros Hc. eapply H6.
-      now eapply name_in_fundefs_bound_var_fundefs.
-    - rewrite image_Empty_set. now eauto with Ensembles_DB.
-  Qed.
-
-
-  Lemma Add_functions_map_eq B fvs σ ζ S σ' ζ' S' l :
-    Add_functions B fvs σ ζ S σ' ζ' S' ->
-    Disjoint _ (FromList l) (name_in_fundefs B) ->
-    map σ l = map σ' l.
-  Proof.
-    intros Hadd HD. induction l; eauto.
-    simpl. rewrite FromList_cons in HD.
-    erewrite Add_functions_σ_eq; [| eassumption |].
-    rewrite IHl. reflexivity.
-    now eauto with Ensembles_DB.
-    intros Hc. eapply HD; eauto.
-  Qed.
-
-  Lemma Add_functions_FunsFVs_Included_alt P B fvs σ ζ S σ' ζ' S' f f' ft fvs' :
-    Add_functions B fvs σ ζ S σ' ζ' S' ->
-    Disjoint _ (FunsFVs ζ) P ->
-    ζ' f = Some (f', ft, fvs') ->
-    fvs' = fvs \/ Disjoint _ (FromList fvs') P.
-  Proof with now eauto with Ensembles_DB.
-    intros Hadd. induction Hadd; intros Hin Heq.
-    - destruct (peq f0 f); subst.
-      + rewrite extend_gss in Heq.
-        inv Heq; eauto.        
-      + rewrite extend_gso in Heq; eauto.
-    - right. eapply Disjoint_Included_l; [| eassumption ].
-      repeat eexists; eauto.
-  Qed.
-
-  Lemma injective_subdomain_Add_functions P B fvs σ ζ S σ' ζ' S'  :
-    Add_functions B fvs σ ζ S σ' ζ' S' ->
-    unique_bindings_fundefs B ->
-    injective_subdomain (Setminus _ P (name_in_fundefs B)) σ ->
-    Disjoint _ (image σ (Setminus _ P (name_in_fundefs B))) (name_in_fundefs B) ->
-    injective_subdomain P σ'.
-  Proof with now eauto with Ensembles_DB.
-    intros Hadd. revert P; induction Hadd; intros P Hun Hinj HD.
-    - inv Hun. eapply injective_subdomain_extend'.
-      eapply IHHadd. eassumption. now rewrite Setminus_Union.
-      rewrite Setminus_Union...
-      intros Hc. eapply Add_functions_image_Included in Hc; [| eassumption ].
-      inv Hc. eapply HD.
-      constructor; eauto. rewrite Setminus_Union in H0; eassumption.
-      left; eauto.
-      eapply H6. eapply name_in_fundefs_bound_var_fundefs. eassumption.
-    - simpl in Hinj. now rewrite Setminus_Empty_set_neut_r in Hinj.
-  Qed.
-  
-  Lemma image_LiftedFuns_Add_functions_Included B fvs σ ζ S σ' ζ' S' x f :
-    Add_functions B fvs σ ζ S σ' ζ' S' ->
-    lifted_name ζ' x = Some f ->
-    In _ (name_in_fundefs B) x ->
-    In _ S f /\ ~ In _ S' f.
-  Proof with now eauto with Ensembles_DB.
-    intros Hadd. induction Hadd; intros Heq Hin.
-    - destruct (peq f0 x); subst.
-      + rewrite lifted_name_extend, extend_gss in Heq. inv Heq.
-        split.
-        eapply Add_functions_free_set_Included; eassumption.
-        intros Hc. inv Hc; eauto.
-      + rewrite lifted_name_extend, extend_gso in Heq; eauto.
-        inv Hin. inv H0; congruence.
-        eapply IHHadd in Heq; eauto. inv Heq.
-        split; eauto. intros Hc. inv Hc. eauto.
-    - inv Hin.
-  Qed.
-    
-  Lemma injective_subdomain_LiftedFuns_Add_functions B fvs σ ζ S σ' ζ' S'  :
-    Add_functions B fvs σ ζ S σ' ζ' S' ->
-    injective_subdomain (name_in_fundefs B) (lifted_name ζ').
-  Proof with now eauto with Ensembles_DB.
-    intros Hadd. induction Hadd.
-    - simpl. rewrite lifted_name_extend. eapply injective_subdomain_extend.
-      eassumption.
-      intros [x [Hin Heq]]; subst. inv Hin.
-      eapply image_LiftedFuns_Add_functions_Included in Hadd; try eassumption.
-      inv Hadd; eauto.
-    - eapply injective_subdomain_Empty_set.
-  Qed.
-
-  Lemma Fundefs_lambda_lift_name_in_fundefs ζ σ B S B' S' :
-    Fundefs_lambda_lift ζ σ B S B' S' ->
-    Included _ (name_in_fundefs B') (Union _ (name_in_fundefs B) (LiftedFuns ζ)).
-  Proof.
-    intros Hadd; induction Hadd; simpl.
-    - assert (Heq := lifted_name_eq _ _ _ _ _ H).
-      assert (Hin : Included _ (Singleton var f') (LiftedFuns ζ)).
-      { eapply Singleton_Included. repeat eexists; eauto. }
-      eapply Union_Included.
-      now eauto with Ensembles_DB.
-      eapply Union_Included. now eauto with Ensembles_DB.
-      eapply Included_trans; now eauto with Ensembles_DB.
-    - now eauto with Ensembles_DB.
-  Qed.
-
-  Lemma bound_var_fun_in_fundefs B f ft xs e :
-    In _ (fun_in_fundefs B) (f, ft, xs, e) ->
-    Included _ (Union _ (Singleton _ f) (Union _ (FromList xs) (bound_var e)))
-             (bound_var_fundefs B).
-  Proof with now eauto with Ensembles_DB.
-    intros Hin; induction B; inv Hin.
-    - inv H. normalize_bound_var...
-    - normalize_bound_var...
-  Qed.
-
-  Lemma unique_bindings_fun_in_fundefs B f ft xs e :
-    In _ (fun_in_fundefs B) (f, ft, xs, e) ->
-    unique_bindings_fundefs B ->
-    unique_bindings e /\
-    ~ In _ (bound_var e) f /\
-    ~ In _ (FromList xs) f /\
-    Disjoint _ (bound_var e) (name_in_fundefs B) /\
-    Disjoint _ (FromList xs) (name_in_fundefs B) /\    
-    Disjoint _ (bound_var e) (FromList xs) /\
-    NoDup xs.
-  Proof with now eauto with Ensembles_DB.
-    intros Hin Hun; induction Hun.
-    -inv Hin.
-     + inv H7. split; [| split; [| split; [| split; [| split]]]]; eauto; simpl.
-       eapply Union_Disjoint_r.
-       eapply Disjoint_Singleton_r; eassumption.
-       eapply Disjoint_Included_r; [| now apply H3 ].
-       now apply name_in_fundefs_bound_var_fundefs.
-       eapply Union_Disjoint_r.
-       eapply Disjoint_Singleton_r; eassumption.
-       eapply Disjoint_Included_r_sym; [| now apply H2 ].
-       now apply name_in_fundefs_bound_var_fundefs.
-     + edestruct IHHun as [Hun' [Hnin1 [Hnin2 [HD1 [HD2 [HD3 Hnd]]]]]].
-       eassumption.
-       split; [| split; [| split; [| split; [| split; [| split ]]]]]; eauto; simpl;
-       eapply bound_var_fun_in_fundefs in H7.
-       eapply Union_Disjoint_r; [| eassumption ].
-       eapply Disjoint_Singleton_r.
-       intros Hc. eapply H0.
-       eapply H7. now eauto.
-       eapply Union_Disjoint_r; [| eassumption ].
-       eapply Disjoint_Singleton_r.
-       intros Hc. eapply H0.
-       eapply H7. now eauto.
-    - inv Hin.
-  Qed.
-
-  Lemma NoDup_app {A} xs ys :
-    NoDup xs -> NoDup ys ->
-    Disjoint A (FromList xs) (FromList ys) ->
-    NoDup (xs ++ ys).
-  Proof with now eauto with Ensembles_DB.
-    revert ys; induction xs; intros ys Hnd1 Hnd2 HD; simpl; eauto.
-    inv Hnd1. rewrite FromList_cons in HD.
-    constructor. intros Hc. eapply in_app_or in Hc. inv Hc; eauto.
-    now eapply HD; constructor; eauto.
-    eapply IHxs; eauto...
-  Qed.
-
-  Lemma bound_var_occurs_free_in_fun_Included f t xs e B :
-    In _ (fun_in_fundefs B) (f, t, xs, e) ->
-    Included var (Union var (bound_var e) (occurs_free e))
-             (Union var (bound_var_fundefs B) (occurs_free_fundefs B)).
-  Proof with now eauto with Ensembles_DB.
-    induction B; intros Hin; inv Hin.
-    - inv H. now eapply bound_var_occurs_free_Fcons_Included.
-    - normalize_bound_var. normalize_occurs_free.
-      eapply Included_trans. eapply IHB. eassumption.
-      eapply Union_Included. now eauto with Ensembles_DB.
-      rewrite Union_assoc.
-      rewrite Union_Setminus_Included; eauto with Ensembles_DB typeclass_instances.
-  Qed.
-
-  Lemma FromList_map_image_FromList {A B} l (f : A -> B):
-    Same_set B (FromList (map f l)) (image f (FromList l)).
-  Proof with now eauto with Ensembles_DB.
-    induction l; simpl.
-    - rewrite !FromList_nil, image_Empty_set...
-    - rewrite !FromList_cons, image_Union, image_Singleton...
-  Qed.
-
-  Lemma map_Add_functions_Disjoint B fvs f g S f' g' S' l :
-    Add_functions B fvs f g S f' g' S' ->
-    Disjoint positive (FromList l) (name_in_fundefs B) ->
-    map f' l = map f l.
-  Proof with now eauto with Ensembles_DB.
-    intros Hadd HD. induction Hadd.
-    - rewrite map_extend_not_In. eapply IHHadd...
-      intros Hc. eapply HD; eauto.
-      constructor; eauto. left; eauto.
-    - reflexivity.
-  Qed.    
-
-  Lemma getlist_length_eq {A} l (vs : list A) rho : 
-    getlist l rho = Some vs ->
-    length l = length vs.
-  Proof.
-    revert vs; induction l; intros vs Hget.
-    - inv Hget. eauto.
-    - simpl in Hget. destruct (M.get a rho); try discriminate.
-      destruct (getlist l rho); try discriminate.
-      inv Hget. simpl. f_equal; eauto.
-  Qed.
-
-  Lemma app_getlist {A} l1 l2 (vs : list A) rho :
-    getlist (l1 ++ l2) rho = Some vs ->
-    exists vs1 vs2,
-      getlist l1 rho = Some vs1 /\
-      getlist l2 rho = Some vs2 /\
-      vs = vs1 ++ vs2.
-  Proof.
-    revert vs. induction l1; intros vs Hget.
-    - simpl in Hget. repeat eexists; eauto.
-    - simpl in Hget.
-      destruct (M.get a rho) eqn:Hgeta; try discriminate.
-      destruct (getlist (l1 ++ l2) rho) eqn:Hgetl; try discriminate.
-      inv Hget.
-      edestruct IHl1 as [vs1 [vs2 [Hget1 [Hget2 Heq]]]].
-      reflexivity.
-      repeat eexists; eauto. simpl.
-      rewrite Hgeta, Hget1. reflexivity.
-      simpl. congruence.
-  Qed.
-
-  Lemma f_eq_subdomain_extend_not_In_S_r' {A} P (f1 f2 : positive -> A) v v' :
-    f_eq_subdomain (Union _ P (Singleton _ v)) f1 (f2 {v ~> v'}) ->
-    ~ In _ P v ->
-    f_eq_subdomain P f1 f2.
-  Proof.
-    intros Heq Hin x y. erewrite <- (extend_gso f2).
-    apply Heq; constructor; eauto.
-    intros Hc. subst. eauto.
-  Qed.
-    
   Lemma Funs_inv_set_lifted k rho rho' rho1 rho2 B1 B1' ζ σ v v' ft ft' xs xs' ys fvs e1 e1' vs  :
     preord_val pr cenv k (Vfun rho1 B1 v) (Vfun rho2 B1' v) ->
 
@@ -1451,52 +376,364 @@ Section Lambda_lifting_correct.
         left. eapply fun_in_fundefs_name_in_fundefs.
         apply find_def_correct. eassumption.
   Qed.
-  
-  Lemma name_in_fundefs_find_def_is_Some f B :
+
+  (** * Lemmas about [Add_functions] *)
+
+  Lemma Add_functions_free_set_Included B fvs ζ σ S ζ' σ' S' :
+    Add_functions B fvs ζ σ S ζ' σ' S' ->
+    Included _ S' S.
+  Proof with now eauto with Ensembles_DB.
+    intros Hadd. induction Hadd...
+  Qed.
+
+  Lemma Add_functions_fvs_eq B fvs σ ζ S σ' ζ' S' f f' ft fvs' :
+    Add_functions B fvs σ ζ S σ' ζ' S' ->
+    ζ' f = Some (f', ft, fvs') ->
     In _ (name_in_fundefs B) f ->
-    exists ft xs e, find_def f B = Some (ft, xs, e).
+    fvs' = fvs.
   Proof.
-    intros Hin. induction B.
-    - destruct (peq v f); simpl; subst.
-      + repeat eexists; eauto.
-        rewrite peq_true. reflexivity.
-      + inv Hin. inv H; congruence.
-        rewrite peq_false; eauto.
+    intros Hadd Heq Hin; induction Hadd.
+    - destruct (peq f f0); subst.
+      + rewrite extend_gss in Heq. inv Heq. eauto.
+      + inv Hin. inv H0; congruence.
+        rewrite extend_gso in Heq; eauto.
     - inv Hin.
   Qed.
 
-  Lemma fun_in_fundefs_Disjoint_bound_Var_occurs_free B f t xs e :
-    fun_in_fundefs B (f, t, xs, e) ->
+  Lemma Add_functions_image_Included P B fvs σ ζ S σ' ζ' S' :
+    Add_functions B fvs σ ζ S σ' ζ' S' ->
+    Included _ (image σ' P) (Union _ (image σ (Setminus _ P (name_in_fundefs B))) (name_in_fundefs B)).
+  Proof with now eauto with Ensembles_DB.
+    intros Hadd. revert P. induction Hadd; intros P.
+    - eapply Included_trans.
+      eapply image_extend_Included'. 
+      eapply Union_Included; [| now eauto with Ensembles_DB ].
+      eapply Included_trans. eapply IHHadd.
+      rewrite Setminus_Union...
+    - now eauto with Ensembles_DB.
+  Qed.
+
+  Lemma Add_functions_LiftedFuns_Included B fvs σ ζ S σ' ζ' S' :
+    Add_functions B fvs σ ζ S σ' ζ' S' ->
+    Included _ (LiftedFuns ζ') (Union _ (LiftedFuns ζ) (Setminus _ S S')).
+  Proof with now eauto with Ensembles_DB.
+    intros Hadd. induction Hadd.
+    - eapply Included_trans.
+      eapply LiftedFuns_extend_Some.
+      eapply Union_Included.
+      eapply Included_trans. now eapply IHHadd.
+      now eauto with Ensembles_DB.
+      eapply Included_Union_preserv_r.
+      eapply Singleton_Included. constructor.
+      eapply Add_functions_free_set_Included; eassumption.
+      intros Hc. inv Hc. eauto.
+    - now eauto with Ensembles_DB.
+  Qed.
+
+  Lemma Add_functions_Funs_Included B fvs σ ζ S σ' ζ' S' :
+    Add_functions B fvs σ ζ S σ' ζ' S' ->
+    Included _ (Funs ζ') (Union _ (Funs ζ) (name_in_fundefs B)).
+  Proof with now eauto with Ensembles_DB.
+    intros Hadd. induction Hadd.
+    - eapply Included_trans.
+      eapply Funs_extend_Some.
+      eapply Union_Included.
+      eapply Included_trans. now eapply IHHadd.
+      now eauto with Ensembles_DB.
+      eapply Included_Union_preserv_r...
+    - now eauto with Ensembles_DB.
+  Qed.
+
+  Lemma Add_functions_FunsFVs_Included_r B fvs σ ζ S σ' ζ' S' :
+    Add_functions B fvs σ ζ S σ' ζ' S' ->
+    Included _ (FunsFVs ζ') (Union _ (FunsFVs ζ) (FromList fvs)).
+  Proof with now eauto with Ensembles_DB.
+    intros Hadd. induction Hadd.
+    - eapply Included_trans.
+      eapply FunsFVs_extend_Some.
+      eapply Union_Included.
+      eapply Included_trans. now eapply IHHadd.
+      now eauto with Ensembles_DB.
+      eapply Included_Union_preserv_r...
+    - now eauto with Ensembles_DB.
+  Qed.
+
+  Lemma Add_functions_FunsFVs_Included_l B fvs σ ζ S σ' ζ' S' :
+    Add_functions B fvs σ ζ S σ' ζ' S' ->
     unique_bindings_fundefs B ->
-    Disjoint _ (bound_var_fundefs B) (occurs_free_fundefs B) ->
-    Disjoint _ (bound_var e) (occurs_free e).
-  Proof.    
-    intros Hin Hun HD; induction B; inv Hun.
-    - assert (Hin' := Hin). inv Hin.
-      + inv H.
-        eapply Disjoint_Included_r.
-        eapply occurs_free_in_fun. eassumption.
-        repeat normalize_bound_var_in_ctx.
-        repeat normalize_occurs_free_in_ctx.
-        normalize_occurs_free.
-        eapply Union_Disjoint_r. eassumption.
-        eapply Union_Disjoint_r. simpl. 
-        eapply Union_Disjoint_r.
-        apply Disjoint_Singleton_r. eassumption.
-        eapply Disjoint_Included_r; [| now eapply H8 ].
-        now apply name_in_fundefs_bound_var_fundefs.
-        now eauto with Ensembles_DB.
-      + eapply IHB; try eassumption.
-        repeat normalize_bound_var_in_ctx.
-        eapply Disjoint_Included_r.
-        eapply occurs_free_fundefs_Fcons_Included. 
-        eapply Union_Disjoint_r.
-        eapply Disjoint_Included_l; [| now apply HD ].
-        now eauto with Ensembles_DB.
-        apply Disjoint_Singleton_r. eassumption.
+    Disjoint _ (Funs ζ) (name_in_fundefs B) ->
+    Included _ (FunsFVs ζ) (FunsFVs ζ').
+  Proof with now eauto with Ensembles_DB.
+    intros Hadd Hun HD. induction Hadd.
+    - inv Hun. eapply Included_trans. eapply IHHadd.
+      eassumption. now eauto with Ensembles_DB.
+      rewrite FunsFVs_extend_Some_eq.
+      now eauto with Ensembles_DB.
+      intros Hc. 
+      eapply Add_functions_Funs_Included in Hc; [| eassumption ].
+      inv Hc. eapply HD. constructor; eauto. left; eauto.
+      eapply H6. apply name_in_fundefs_bound_var_fundefs. eassumption.
+    - now eauto with Ensembles_DB.
+  Qed.
+
+  Lemma Add_functions_σ_eq B fvs σ ζ S σ' ζ' S' :
+    Add_functions B fvs σ ζ S σ' ζ' S' ->
+    f_eq_subdomain (Complement _ (name_in_fundefs B)) σ σ'.
+  Proof.
+    intros Hadd. induction Hadd; simpl.
+    - eapply f_eq_subdomain_extend_not_In_S_r.
+      intros Hc; apply Hc. eauto.
+      eapply f_eq_subdomain_antimon; [| eassumption ].
+      now eauto with Ensembles_DB.
+    - reflexivity.
+  Qed.
+
+  Lemma Add_functions_lifted_name_Disjoint B fvs σ ζ S σ' ζ' S' :
+    Add_functions B fvs σ ζ S σ' ζ' S' ->
+    unique_bindings_fundefs B ->
+    Disjoint _ (LiftedFuns ζ) S ->
+    Disjoint _ (image (lifted_name ζ') (name_in_fundefs B))
+             (image (lifted_name ζ') (Complement _ (name_in_fundefs B))).
+  Proof.
+    intros Hadd Hun HD. induction Hadd; simpl.
+    - inv Hun. rewrite image_Union. apply Union_Disjoint_l.
+      rewrite image_Singleton.
+      rewrite !lifted_name_extend, !extend_gss.
+      rewrite image_extend_not_In_S; eauto.
+      constructor. intros x Hc. inv Hc. inv H0.
+      destruct H1 as [x' [Hin Heq]].
+      assert (Hin' : In _ (LiftedFuns ζ') f').
+      now repeat eexists; eauto.
+      eapply Add_functions_LiftedFuns_Included in Hin'; [| eassumption ].
+      inv Hin'. eapply HD.  constructor; eauto.
+      eapply Add_functions_free_set_Included; eassumption.
+      inv H0; eauto.
+      eapply Disjoint_Included; [| | now apply IHHadd ].
+      rewrite lifted_name_extend. rewrite image_extend_not_In_S; eauto.
+      apply image_monotonic...
+      now eauto with Ensembles_DB.
+      rewrite lifted_name_extend. rewrite image_extend_not_In_S; eauto.
+      reflexivity. intros Hc. eapply H6.
+      now eapply name_in_fundefs_bound_var_fundefs.
+    - rewrite image_Empty_set. now eauto with Ensembles_DB.
+  Qed.
+
+
+  Lemma Add_functions_map_eq B fvs σ ζ S σ' ζ' S' l :
+    Add_functions B fvs σ ζ S σ' ζ' S' ->
+    Disjoint _ (FromList l) (name_in_fundefs B) ->
+    map σ l = map σ' l.
+  Proof.
+    intros Hadd HD. induction l; eauto.
+    simpl. rewrite FromList_cons in HD.
+    erewrite Add_functions_σ_eq; [| eassumption |].
+    rewrite IHl. reflexivity.
+    now eauto with Ensembles_DB.
+    intros Hc. eapply HD; eauto.
+  Qed.
+
+  Lemma Add_functions_FunsFVs_Included_alt P B fvs σ ζ S σ' ζ' S' f f' ft fvs' :
+    Add_functions B fvs σ ζ S σ' ζ' S' ->
+    Disjoint _ (FunsFVs ζ) P ->
+    ζ' f = Some (f', ft, fvs') ->
+    fvs' = fvs \/ Disjoint _ (FromList fvs') P.
+  Proof with now eauto with Ensembles_DB.
+    intros Hadd. induction Hadd; intros Hin Heq.
+    - destruct (peq f0 f); subst.
+      + rewrite extend_gss in Heq.
+        inv Heq; eauto.        
+      + rewrite extend_gso in Heq; eauto.
+    - right. eapply Disjoint_Included_l; [| eassumption ].
+      repeat eexists; eauto.
+  Qed.
+
+  Lemma Add_functions_injective_subdomain P B fvs σ ζ S σ' ζ' S'  :
+    Add_functions B fvs σ ζ S σ' ζ' S' ->
+    unique_bindings_fundefs B ->
+    injective_subdomain (Setminus _ P (name_in_fundefs B)) σ ->
+    Disjoint _ (image σ (Setminus _ P (name_in_fundefs B))) (name_in_fundefs B) ->
+    injective_subdomain P σ'.
+  Proof with now eauto with Ensembles_DB.
+    intros Hadd. revert P; induction Hadd; intros P Hun Hinj HD.
+    - inv Hun. eapply injective_subdomain_extend'.
+      eapply IHHadd. eassumption. now rewrite Setminus_Union.
+      rewrite Setminus_Union...
+      intros Hc. eapply Add_functions_image_Included in Hc; [| eassumption ].
+      inv Hc. eapply HD.
+      constructor; eauto. rewrite Setminus_Union in H0; eassumption.
+      left; eauto.
+      eapply H6. eapply name_in_fundefs_bound_var_fundefs. eassumption.
+    - simpl in Hinj. now rewrite Setminus_Empty_set_neut_r in Hinj.
+  Qed.
+  
+  Lemma Add_functions_image_LiftedFuns_Included B fvs σ ζ S σ' ζ' S' x f :
+    Add_functions B fvs σ ζ S σ' ζ' S' ->
+    lifted_name ζ' x = Some f ->
+    In _ (name_in_fundefs B) x ->
+    In _ S f /\ ~ In _ S' f.
+  Proof with now eauto with Ensembles_DB.
+    intros Hadd. induction Hadd; intros Heq Hin.
+    - destruct (peq f0 x); subst.
+      + rewrite lifted_name_extend, extend_gss in Heq. inv Heq.
+        split.
+        eapply Add_functions_free_set_Included; eassumption.
+        intros Hc. inv Hc; eauto.
+      + rewrite lifted_name_extend, extend_gso in Heq; eauto.
+        inv Hin. inv H0; congruence.
+        eapply IHHadd in Heq; eauto. inv Heq.
+        split; eauto. intros Hc. inv Hc. eauto.
     - inv Hin.
-  Qed.       
+  Qed.
     
+  Lemma Add_functions_injective_subdomain_LiftedFuns B fvs σ ζ S σ' ζ' S'  :
+    Add_functions B fvs σ ζ S σ' ζ' S' ->
+    injective_subdomain (name_in_fundefs B) (lifted_name ζ').
+  Proof with now eauto with Ensembles_DB.
+    intros Hadd. induction Hadd.
+    - simpl. rewrite lifted_name_extend. eapply injective_subdomain_extend.
+      eassumption.
+      intros [x [Hin Heq]]; subst. inv Hin.
+      eapply Add_functions_image_LiftedFuns_Included in Hadd; try eassumption.
+      inv Hadd; eauto.
+    - eapply injective_subdomain_Empty_set.
+  Qed.
+
+  Lemma Add_functions_map_Disjoint B fvs f g S f' g' S' l :
+    Add_functions B fvs f g S f' g' S' ->
+    Disjoint positive (FromList l) (name_in_fundefs B) ->
+    map f' l = map f l.
+  Proof with now eauto with Ensembles_DB.
+    intros Hadd HD. induction Hadd.
+    - rewrite map_extend_not_In. eapply IHHadd...
+      intros Hc. eapply HD; eauto.
+      constructor; eauto. left; eauto.
+    - reflexivity.
+  Qed.
+
+  (** * Lemmas about [Exp_lambda_lift] and [Fundefs_lambda_lift] *)
+
+  Lemma Fundefs_lambda_lift_name_in_fundefs ζ σ B S B' S' :
+    Fundefs_lambda_lift ζ σ B S B' S' ->
+    Included _ (name_in_fundefs B') (Union _ (name_in_fundefs B) (LiftedFuns ζ)).
+  Proof.
+    intros Hadd; induction Hadd; simpl.
+    - assert (Heq := lifted_name_eq _ _ _ _ _ H).
+      assert (Hin : Included _ (Singleton var f') (LiftedFuns ζ)).
+      { eapply Singleton_Included. repeat eexists; eauto. }
+      eapply Union_Included.
+      now eauto with Ensembles_DB.
+      eapply Union_Included. now eauto with Ensembles_DB.
+      eapply Included_trans; now eauto with Ensembles_DB.
+    - now eauto with Ensembles_DB.
+  Qed.
+
+  Lemma Lambda_lift_free_set_Included_mut :
+    (forall e ζ σ S e' S',
+       Exp_lambda_lift ζ σ e S e' S' ->
+       Included _ S' S) /\
+    (forall B ζ σ S B' S',
+       Fundefs_lambda_lift ζ σ B S B' S' ->
+       Included _ S' S).
+  Proof with now eauto with Ensembles_DB.
+    exp_defs_induction IHe IHl IHB; intros; inv H; try now eauto with Ensembles_DB.
+    - eapply Included_trans. now eapply IHl; eauto.
+      eapply IHe; eauto.
+    - eapply Included_trans. now eapply IHe; eauto.
+      eapply Included_trans. now eapply IHB; eauto.
+      eapply Add_functions_free_set_Included; eauto.
+    - eapply Included_trans. now eapply IHB; eauto.
+      eapply Included_trans. now eapply IHe; eauto.
+      now eauto with Ensembles_DB.
+  Qed.
+
+  Corollary Exp_Lambda_lift_free_set_Included :
+    forall e ζ σ S e' S',
+      Exp_lambda_lift ζ σ e S e' S' ->
+      Included _ S' S.
+  Proof.
+    destruct Lambda_lift_free_set_Included_mut; eauto.
+  Qed.
+
+  Corollary Fundefs_Lambda_lift_free_set_Included :
+    forall B ζ σ S B' S',
+      Fundefs_lambda_lift ζ σ B S B' S' ->
+      Included _ S' S.
+  Proof.
+    destruct Lambda_lift_free_set_Included_mut; eauto.
+  Qed.
+  
+  Lemma Fundefs_lambda_lift_find_def σ ζ S1 B1 S2 B2 f t xs1 e1 f' t' fvs :
+    Fundefs_lambda_lift ζ σ B1 S1 B2 S2 ->
+    ζ f = Some (f', t', fvs) ->
+    Disjoint _ (bound_var_fundefs B1) (LiftedFuns ζ) ->
+    injective_subdomain (name_in_fundefs B1) (lifted_name ζ) ->
+    find_def f B1 = Some (t, xs1, e1) ->
+    exists (xs1' ys : list var) (e2 : exp) S2 S2',
+      find_def f B2 = Some (t, xs1', (Eapp f' t' (xs1' ++ map σ fvs))) /\
+      find_def f' B2 = Some (t', xs1 ++ ys, e2) /\
+      NoDup ys /\ NoDup xs1' /\
+      length xs1 = length xs1' /\
+      length ys = length fvs /\
+      Included _ S2 S1 /\
+      Included _ (FromList ys) S1 /\
+      Included _ (FromList xs1') S1 /\
+      Disjoint _ (FromList ys) S2 /\
+      Disjoint _ (FromList xs1') S2 /\
+      Disjoint _ (FromList xs1') (FromList ys) /\
+      Exp_lambda_lift ζ (σ <{ xs1 ++ fvs ~> xs1 ++ ys }>) e1 S2 e2 S2'.
+  Proof with now eauto with Ensembles_DB.
+    intros Hll. induction Hll; intros Heq HD Hinj Hdef.
+    - assert (Heq' := lifted_name_eq _ _ _ _ _ Heq).
+      simpl in Hdef. destruct (M.elt_eq f f0); subst.
+      + rewrite Heq in H; inv H. inv Hdef.
+        exists xs', ys, e'. do 2 eexists.
+        split; [| split; [| split; [| split; [| split; [| split; [| split; [| split; [| split; [| split; [| split; [| split]]]]]]]]]]];
+        [ | | | | | | | | | | | | eassumption ]; eauto.
+        * simpl. rewrite peq_false, peq_true. reflexivity.
+          intros Hc. subst. eapply HD. constructor; eauto.
+          repeat eexists; eauto.
+        * simpl. rewrite peq_true. reflexivity.
+        * now eauto with Ensembles_DB.
+        * eapply Included_trans; [ eassumption |]...
+        * now eauto with Ensembles_DB.
+        * now eauto with Ensembles_DB.
+        * eapply Disjoint_Included_l; [ eassumption |]...
+      + destruct IHHll as (xs1' & ys' & e2 & S2 & S2' & Hf1 & Hf2 & Hnd1 & Hnd2
+                                & Heq1 & Heq2 & Hinc1 & Hinc2 & Hinc3 & Hd1 & Hd2 & Hd3 & Hexp).
+        eassumption. normalize_bound_var_in_ctx...
+        eapply injective_subdomain_antimon. eassumption.
+        now eauto with Ensembles_DB. eassumption.
+        eexists xs1', ys', e2. do 2 eexists.
+        split; [| split; [| split; [| split; [| split; [| split; [| split; [| split; [| split; [| split; [| split; [| split]]]]]]]]]]];
+        [ | | | | | | | | | | | | eassumption ]; eauto.
+        * simpl. rewrite peq_false; eauto. rewrite peq_false; now eauto.
+          intros Hc. subst. eapply HD. constructor.
+          constructor 2. apply name_in_fundefs_bound_var_fundefs.
+          eapply fun_in_fundefs_name_in_fundefs. eapply find_def_correct.
+          eassumption. eexists.
+          split; repeat eexists; now unfold lifted_name; rewrite H; eauto.
+        * simpl. rewrite peq_false; eauto. rewrite peq_false; eauto.
+          intros Hc. subst. eapply HD. constructor. now eauto.
+          now repeat eexists; eauto.
+          intros Hc; subst. eapply n. eapply Hinj.
+          constructor 2. eapply fun_in_fundefs_name_in_fundefs.
+          eapply find_def_correct. eassumption.
+          now simpl; eauto. erewrite !lifted_name_eq; eauto.
+        * eapply Included_trans. eassumption.
+          eapply Included_trans. eapply Exp_Lambda_lift_free_set_Included.
+          eassumption.
+          now eauto with Ensembles_DB.
+        * eapply Included_trans. eassumption.
+          eapply Included_trans.
+          eapply Exp_Lambda_lift_free_set_Included; now eauto.
+          now eauto with Ensembles_DB.
+        * eapply Included_trans. eassumption.
+          eapply Included_trans.
+          eapply Exp_Lambda_lift_free_set_Included; now eauto.
+          now eauto with Ensembles_DB.
+    - inv Hdef.
+  Qed.
+      
   Lemma Fundefs_lambda_lift_correct k rho rho' B1 B1' B2 B2' σ ζ σ1 ζ1 σ2 ζ2 S
         S1' S1'' S1''' S2' S2'' S2''' fvs e:
     (* The IH for expressions *)
@@ -1541,16 +778,20 @@ Section Lambda_lifting_correct.
      (* The domain of ζ is disjoint with the bound variables *)
      Disjoint var (Funs ζ) (bound_var_fundefs B1) ->
 
-     (* The free variables of the funs in ζ are disjoint with the bound variables *) 
+     (* The free variables of the funs in ζ are disjoint from the bound variables *) 
      Disjoint var (FunsFVs ζ) (bound_var_fundefs B1) ->
      Disjoint var (FunsFVs ζ) (bound_var_fundefs B2) ->
 
+     (* The bound variables and the free variables are disjoint *)
      Disjoint _ (bound_var_fundefs B1) (occurs_free_fundefs B1) ->
 
+     (* The free variables are in the environment *)
      binding_in_map (Union _ (occurs_free (Efun B1 e)) (FunsFVs ζ)) rho ->
 
+     (** ζ1 and ζ2 are equal in a [name_in_fundefs B2] *) 
      f_eq_subdomain (name_in_fundefs B2) ζ1 ζ2 ->
 
+     (** The invariant hold for the initial environments **)
      preord_env_P_inj pr cenv (Union _ (occurs_free (Efun B1 e)) (FunsFVs ζ)) k σ rho rho' ->
      Funs_inv k rho rho' σ ζ ->
      
@@ -1560,7 +801,7 @@ Section Lambda_lifting_correct.
      Disjoint var (FromList fvs) (bound_var_fundefs B2) ->
 
      Included _ (name_in_fundefs B2) (name_in_fundefs B1) ->
-
+     
      Add_functions B1 fvs σ ζ S σ1 ζ1 S1' ->
      Included _ S1'' S1' ->
      Fundefs_lambda_lift ζ1 σ1 B1 S1'' B1' S1''' ->
@@ -1568,7 +809,8 @@ Section Lambda_lifting_correct.
      Add_functions B2 fvs σ ζ S σ2 ζ2 S2' ->
      Included _ S2'' S2' ->
      Fundefs_lambda_lift ζ1 σ1 B2 S2'' B2' S2''' ->
-     
+
+     (** The invariants hold for the final environments **)
      preord_env_P_inj pr cenv (Union _ (Union _ (occurs_free (Efun B1 e)) (name_in_fundefs B2)) (FunsFVs ζ1))
                       k σ2 (def_funs B1 B2 rho rho) (def_funs B1' B2' rho' rho') /\
      Funs_inv k (def_funs B1 B2 rho rho) (def_funs B1' B2' rho' rho') σ2 ζ2.
@@ -1625,7 +867,7 @@ Section Lambda_lifting_correct.
         eapply Disjoint_Included_r_sym. eapply Add_functions_LiftedFuns_Included. eassumption.
         eapply Union_Disjoint_l. eapply Disjoint_Included_r; [| now apply Hlf1 ]...
         eapply Disjoint_Included; [| | now apply Hf1]...
-        eapply injective_subdomain_LiftedFuns_Add_functions. eassumption. eassumption.
+        eapply Add_functions_injective_subdomain_LiftedFuns; eassumption. eassumption.
         (* Various useful assertions *)
         assert (Hfree : Included _ (occurs_free e1)
                                  (Union var (FromList xs1)
@@ -1908,7 +1150,7 @@ Section Lambda_lifting_correct.
         eapply Disjoint_Included_r_sym. eapply Add_functions_LiftedFuns_Included. eassumption.
         eapply Union_Disjoint_l. eapply Disjoint_Included_r; [| now apply Hlf1 ]...
         eapply Disjoint_Included; [| | now apply Hf1]...
-        eapply injective_subdomain_LiftedFuns_Add_functions. eassumption.
+        eapply Add_functions_injective_subdomain_LiftedFuns. eassumption.
         assert (Hinc' : Included M.elt (FromList fvs0)
                                 (Union var (occurs_free (Efun B1 e)) (FunsFVs ζ))).
         { eapply Included_trans with (s2 := FunsFVs ζ1).
@@ -2020,87 +1262,325 @@ Section Lambda_lifting_correct.
       eapply Included_Union_compat. reflexivity. eassumption.
       intros x Hin'. inv Hin'; eauto. inv H; eauto.
   Qed.
-  
+
+  Corollary Fundefs_lambda_lift_correct_cor k rho rho' B1 B1' σ ζ σ1 ζ1 S
+        S1' S1'' S1''' fvs e:
+    (* The IH for expressions *)
+     (forall m : nat,
+        m < k ->
+        forall (e : exp) (rho rho' : env)
+          (ζ : var -> option (var * fTag * list var)) 
+          (σ : var -> var) (S : Ensemble var) (e' : exp) 
+          (S' : Ensemble var),
+        unique_bindings e ->
+        Disjoint var (image σ (Union _ (occurs_free e) (FunsFVs ζ)))
+                 (Union var S (Union _ (bound_var e) (LiftedFuns ζ))) ->
+        Disjoint var S (Union var (bound_var e) (occurs_free e)) ->
+        Disjoint var (LiftedFuns ζ) (Union _ S (bound_var e)) ->
+        Disjoint var (Funs ζ) (bound_var e) ->
+        Disjoint var (FunsFVs ζ) (bound_var e) ->
+        Disjoint _ (bound_var e) (occurs_free e) ->
+        binding_in_map (Union _ (occurs_free e) (FunsFVs ζ)) rho ->
+        preord_env_P_inj pr cenv (Union _ (occurs_free e) (FunsFVs ζ)) m σ rho rho' ->
+        Funs_inv m rho rho' σ ζ ->
+        Exp_lambda_lift ζ σ e S e' S' ->
+        preord_exp pr cenv m (e, rho) (e', rho')) ->
+
+     (* Unique bindings *)
+     unique_bindings_fundefs B1 ->
+
+     (* The image of σ is neither in the free set nor in the set of bound variables *)
+     Disjoint var (image σ (Union _ (occurs_free (Efun B1 e)) (FunsFVs ζ)))
+              (Union var S (Union _ (bound_var_fundefs B1) (LiftedFuns ζ))) ->
+
+     (* The free set is disjoint from the set of bound and free variables *)
+     Disjoint var S (Union var (bound_var_fundefs B1) (occurs_free_fundefs B1)) ->
+
+     (* The names of lifted functions is neither in the free set nor in the set of bound variables*) 
+     Disjoint var (LiftedFuns ζ) (Union _ S (bound_var_fundefs B1)) ->
+
+     (* The domain of ζ is disjoint with the bound variables *)
+     Disjoint var (Funs ζ) (bound_var_fundefs B1) ->
+
+     (* The free variables of the funs in ζ are disjoint from the bound variables *) 
+     Disjoint var (FunsFVs ζ) (bound_var_fundefs B1) ->
+
+     (* The free and bound variables are disjoint *)
+     Disjoint _ (bound_var_fundefs B1) (occurs_free_fundefs B1) ->
+
+     (* All the free variables are in the map *)
+     binding_in_map (Union _ (occurs_free (Efun B1 e)) (FunsFVs ζ)) rho ->
+
+     (* The invariants hold in the initial environment *)
+     preord_env_P_inj pr cenv (Union _ (occurs_free (Efun B1 e)) (FunsFVs ζ)) k σ rho rho' ->
+     Funs_inv k rho rho' σ ζ ->
+     
+     NoDup fvs ->
+     Included _ (FromList fvs) (occurs_free_fundefs B1) ->
+     Disjoint var (FromList fvs) (bound_var_fundefs B1) ->
+     
+     Add_functions B1 fvs σ ζ S σ1 ζ1 S1' ->
+     Included _ S1'' S1' ->
+     Fundefs_lambda_lift ζ1 σ1 B1 S1'' B1' S1''' ->
+     
+     (* The invariants hold in the final environment *)
+     preord_env_P_inj pr cenv (Union _ (Union _ (occurs_free (Efun B1 e)) (name_in_fundefs B1)) (FunsFVs ζ1))
+                      k σ1 (def_funs B1 B1 rho rho) (def_funs B1' B1' rho' rho') /\
+     Funs_inv k (def_funs B1 B1 rho rho) (def_funs B1' B1' rho' rho') σ1 ζ1.
+  Proof.
+    intros. eapply Fundefs_lambda_lift_correct; eauto.
+    reflexivity. reflexivity.
+  Qed.
+
+  Lemma Exp_lambda_lift_Ecase ζ σ x P S e S' :
+    Exp_lambda_lift ζ σ (Ecase x P) S e S' ->
+    exists P', e = Ecase (σ x) P' /\
+          Forall2 (fun p p' : cTag * exp => fst p = fst p') P P'.
+  Proof.
+    revert S S' e; induction P; intros S S' e Hexp; inv Hexp.
+    - eexists; eauto.
+    - eapply IHP in H8. edestruct H8 as [P'' [Heq Hall]]. inv Heq.
+      eexists; eauto.
+  Qed.
+
   Lemma Exp_lambda_lift_correct k rho rho' ζ σ e S e' S' :
     (* The expression has unique bindings *)
     unique_bindings e ->
-    (* The substitution is injective *)
-    injective_subdomain (occurs_free e) σ ->
     (* The new free variable names are fresh *)
-    Disjoint _ (image σ (occurs_free e)) (Union _ S (bound_var e)) ->
+    Disjoint _ (image σ (Union _ (occurs_free e) (FunsFVs ζ)))
+             (Union _ S (Union _ (bound_var e) (LiftedFuns ζ))) ->
     (* The fresh set is fresh *)
     Disjoint _ S (Union _ (bound_var e) (occurs_free e)) ->
     (* The new function names for lifted functions are fresh *)
-    Disjoint _ (LiftedFuns ζ) (bound_var e) ->
+    Disjoint _ (LiftedFuns ζ) (Union _ S (bound_var e)) ->
+    (* The names of the (already defined) functions are disjoint from the bound variables of the expression *)
     Disjoint _ (Funs ζ) (bound_var e) ->
+    (* The free variables of a function are disjoint from the bound variables of the expression *)
     Disjoint _ (FunsFVs ζ) (bound_var e) ->
-    Disjoint _ (image σ (FunsFVs ζ)) (bound_var e) ->
-    preord_env_P_inj pr cenv (occurs_free e) k σ rho rho' ->
+    (* The bound variables of the expression are disjoint from the free variables *)
+    Disjoint _ (bound_var e) (occurs_free e) ->
+    (* All the free variables are in the environment *)
+    binding_in_map (Union _ (occurs_free e) (FunsFVs ζ)) rho ->
+    (* The environments are related *)
+    preord_env_P_inj pr cenv (Union _ (occurs_free e) (FunsFVs ζ)) k σ rho rho' ->
+    (* The invariant about lifted functions hold*)
     Funs_inv k rho rho' σ ζ ->
+    (* e' is the translation of e*)
     Exp_lambda_lift ζ σ e S e' S' ->
+    (* e and e' are related *)
     preord_exp pr cenv k (e, rho) (e', rho').
   Proof with now eauto with Ensembles_DB.
     revert e rho rho' ζ σ S e' S'; induction k as [k IHk] using lt_wf_rec1.
     induction e using exp_ind';
-      intros rho rho' ζ σ S e' S' Hun Hinj HD1 HD2 HD3 HD4 HD5 HD6 Henv Hinv Hll;
+      intros rho rho' ζ σ S e' S' Hun Him Hf Hlf Hfun Hfvs HD Hin Henv Hinv Hll;
       inv Hll.
     - inv Hun. eapply preord_exp_const_compat.
       + eapply Forall2_preord_var_env_map. eassumption.
         normalize_occurs_free...
-      + assert (Hinj' : injective_subdomain (Union _ (occurs_free e) (Singleton _ v))
-                                            (σ {v ~> v})).
-        { eapply injective_subdomain_antimon.
-          eapply injective_subdomain_extend.
-          eassumption.
-          intros Hc. eapply HD1. constructor.
-          eapply image_monotonic; [| eassumption ]... 
-          now eauto.
-          apply Union_Included;
-            [ rewrite Union_commut; now apply occurs_free_Econstr_Included |]...
-        } 
-        intros vs1 vs2 Hall. eapply IHe; [ eassumption | | | | | | | | | | eassumption ].
-        * eapply injective_subdomain_antimon; [ eassumption |]...
+      + intros vs1 vs2 Hall. eapply IHe; [ eassumption | | | | | | | | | | eassumption ].
         * eapply Disjoint_Included_l. now eapply image_extend_Included'.
           eapply Union_Disjoint_l.
-          rewrite occurs_free_Econstr in HD1.
-          eapply Disjoint_Included; [ | | now apply HD1 ].
-          normalize_bound_var... apply image_monotonic...
+          rewrite occurs_free_Econstr in Him.
+          eapply Disjoint_Included; [ | | now apply Him ].
+          normalize_bound_var...
+          apply image_monotonic. rewrite Setminus_Union_distr...
           eapply Union_Disjoint_r.
           eapply Disjoint_Included_l_sym; [| eassumption ]...
-          eapply Disjoint_Singleton_l. eassumption.
+          eapply Disjoint_Singleton_l. intros Hc. inv Hc. now eauto.
+          eapply Hlf. now constructor; eauto.
         * eapply Disjoint_Included_r; [| eassumption ].
           now apply bound_var_occurs_free_Econstr_Included.
         * repeat normalize_bound_var_in_ctx...
         * repeat normalize_bound_var_in_ctx...
         * repeat normalize_bound_var_in_ctx...
-        * rewrite image_extend_not_In_S. repeat normalize_bound_var_in_ctx...
-          intros Hc. eapply HD5. constructor; eauto.
+        * eapply Disjoint_Included_r. now apply occurs_free_Econstr_Included.
+          eapply Union_Disjoint_r.
+          eapply Disjoint_Included_l ; [| now apply HD].
+          normalize_bound_var... now apply Disjoint_Singleton_r.
+        * eapply binding_in_map_antimon; [| eapply binding_in_map_set; eassumption ]. 
+          apply Union_Included; [| now eauto with Ensembles_DB ].
+          rewrite Union_commut, Union_assoc.
+          apply Included_Union_preserv_l.
+          normalize_occurs_free. rewrite Union_assoc.
+          rewrite Union_Setminus_Included;
+            now eauto with Ensembles_DB typeclass_instances.
         * eapply preord_env_P_inj_set_alt.
           eapply preord_env_P_inj_antimon. eassumption.
-          normalize_occurs_free...
+          rewrite Setminus_Union_distr; normalize_occurs_free...
           rewrite preord_val_eq. constructor. reflexivity.
           now apply Forall2_Forall2_asym_included.
-          eassumption.
+          intros Hc. eapply Him. constructor; eauto.
+          eapply image_monotonic; [| eassumption ].
+          rewrite Setminus_Union_distr; normalize_occurs_free...
         * eapply Funs_inv_set.
-          intros Hc. eapply HD4. now constructor; eauto.
-          intros Hc. eapply HD3. now constructor; eauto.
-          intros Hc. eapply HD5. now constructor; eauto.
-          intros Hc. eapply HD6. now constructor; eauto.
+          intros Hc. eapply Hfun. now constructor; eauto.
+          intros Hc. eapply Hlf. now constructor; eauto.
+          intros Hc. eapply Hfvs. now constructor; eauto.
+          intros Hc. eapply Him. constructor; eauto.
+          eapply image_monotonic; [| eassumption ]...
           eassumption.
-    - admit.
-    - admit.
-    - admit.
-    - inv Hun. eapply preord_exp_fun_compat.
-      eapply IHe; [ eassumption | | | | | | | | | | eassumption ].
-      + admit.
-      + admit.
-      + admit.
-      + admit.
-      + admit.
-      + admit.
-      + admit.
-      + admit.
-      + admit.
+    - eapply preord_exp_case_nil_compat.
+    - inv Hun. edestruct Exp_lambda_lift_Ecase as [P'' [Heq Hall]]; eauto. inv Heq.
+      eapply preord_exp_case_cons_compat; eauto.
+      + eapply Henv. left; eauto.
+      + eapply IHe; eauto.
+        * eapply Disjoint_Included; [| | now apply Him ].
+          normalize_bound_var...
+          apply image_monotonic. normalize_occurs_free...
+        * eapply Disjoint_Included_r; [ | now eapply Hf ].
+          normalize_occurs_free. normalize_bound_var...
+        * eapply Disjoint_Included_r; [ | now eapply Hlf ].
+          normalize_bound_var...
+        * eapply Disjoint_Included_r; [ | now eapply Hfun ].
+          normalize_bound_var...
+        * eapply Disjoint_Included_r; [ | now eapply Hfvs ].
+          normalize_bound_var...
+        * eapply Disjoint_Included; [ | | now eapply HD ].
+          normalize_occurs_free... normalize_bound_var...
+        * eapply binding_in_map_antimon; [| eassumption ].
+          normalize_occurs_free...
+        * eapply preord_env_P_inj_antimon. eassumption.
+          normalize_occurs_free...
+      + assert (Hinc : Included _ S'0 S).
+        { eapply Exp_Lambda_lift_free_set_Included; eauto. }
+        eapply IHe0; eauto.
+        * eapply Disjoint_Included; [| | now apply Him ].
+          normalize_bound_var...
+          apply image_monotonic. normalize_occurs_free...
+        * eapply Disjoint_Included; [ | eassumption | now eapply Hf ].
+          normalize_occurs_free. normalize_bound_var...
+        * eapply Disjoint_Included_r; [ | now eapply Hlf ].
+          normalize_bound_var...
+        * eapply Disjoint_Included_r; [ | now eapply Hfun ].
+          normalize_bound_var...
+        * eapply Disjoint_Included_r; [ | now eapply Hfvs ].
+          normalize_bound_var...
+        * eapply Disjoint_Included; [ | | now eapply HD ].
+          normalize_occurs_free... normalize_bound_var...
+        * eapply binding_in_map_antimon; [| eassumption ].
+          normalize_occurs_free...
+        * eapply preord_env_P_inj_antimon. eassumption.
+          normalize_occurs_free...
+    - inv Hun. eapply preord_exp_proj_compat.
+      + eapply Henv. left. normalize_occurs_free...
+      + intros vs1 vs2 Hall. eapply IHe; [ eassumption | | | | | | | | | | eassumption ].
+        * eapply Disjoint_Included_l. now eapply image_extend_Included'.
+          eapply Union_Disjoint_l.
+          rewrite occurs_free_Eproj in Him.
+          eapply Disjoint_Included; [ | | now apply Him ].
+          normalize_bound_var...
+          apply image_monotonic. rewrite Setminus_Union_distr...
+          eapply Union_Disjoint_r.
+          eapply Disjoint_Included_l_sym; [| eassumption ]...
+          eapply Disjoint_Singleton_l. intros Hc. inv Hc. now eauto.
+          eapply Hlf. now constructor; eauto.
+        * eapply Disjoint_Included_r; [| eassumption ].
+          now apply bound_var_occurs_free_Eproj_Included.
+        * repeat normalize_bound_var_in_ctx...
+        * repeat normalize_bound_var_in_ctx...
+        * repeat normalize_bound_var_in_ctx...
+        * eapply Disjoint_Included_r. now apply occurs_free_Eproj_Included.
+          eapply Union_Disjoint_r.
+          eapply Disjoint_Included_l ; [| now apply HD].
+          normalize_bound_var... now apply Disjoint_Singleton_r.
+        * eapply binding_in_map_antimon; [| eapply binding_in_map_set; eassumption ]. 
+          apply Union_Included; [| now eauto with Ensembles_DB ].
+          rewrite Union_commut, Union_assoc.
+          apply Included_Union_preserv_l.
+          normalize_occurs_free. rewrite Union_assoc.
+          rewrite Union_Setminus_Included;
+            now eauto with Ensembles_DB typeclass_instances.
+        * eapply preord_env_P_inj_set_alt.
+          eapply preord_env_P_inj_antimon. eassumption.
+          rewrite Setminus_Union_distr; normalize_occurs_free...
+          eassumption.
+          intros Hc. eapply Him. constructor; eauto.
+          eapply image_monotonic; [| eassumption ].
+          rewrite Setminus_Union_distr; normalize_occurs_free...
+        * eapply Funs_inv_set.
+          intros Hc. eapply Hfun. now constructor; eauto.
+          intros Hc. eapply Hlf. now constructor; eauto.
+          intros Hc. eapply Hfvs. now constructor; eauto.
+          intros Hc. eapply Him. constructor; eauto.
+          eapply image_monotonic; [| eassumption ]...
+          eassumption.
+    - assert (Hinc : Included _ S'' S).
+      { eapply Included_trans.
+        now eapply Fundefs_Lambda_lift_free_set_Included; eauto.
+        now eapply Add_functions_free_set_Included; eauto. }
+      inv Hun. eapply preord_exp_fun_compat.
+      repeat normalize_bound_var_in_ctx.
+      edestruct Fundefs_lambda_lift_correct_cor; eauto; eauto with Ensembles_DB.
+      + eapply Disjoint_Included_r; [| now apply Hf ].
+        rewrite <- bound_var_Efun.
+        now apply bound_var_occurs_free_fundefs_Efun_Included.
+      + eapply Disjoint_Included; [| | now apply HD].
+        normalize_occurs_free... now eauto with Ensembles_DB.
+      + apply Disjoint_sym. eapply Disjoint_Included; [| | now apply HD ].
+        normalize_occurs_free... now eauto with Ensembles_DB. 
+      + eapply IHe; eauto.
+        * eapply Disjoint_Included_r.
+          apply Included_Union_compat. eassumption.
+          eapply Included_Union_compat. reflexivity.
+          eapply Add_functions_LiftedFuns_Included. eassumption.
+          eapply Disjoint_Included_l. 
+          eapply Add_functions_image_Included. eassumption.
+          apply Union_Disjoint_l.
+          eapply Disjoint_Included; [| | now apply Him ].
+          now eauto 10 with Ensembles_DB.
+          apply image_monotonic. rewrite Setminus_Union_distr.
+          eapply Union_Included. normalize_occurs_free...
+          apply Setminus_Included_Included_Union. normalize_occurs_free.
+          eapply Included_trans. eapply Add_functions_FunsFVs_Included_r.
+          eassumption. now eauto with Ensembles_DB.
+          eapply Disjoint_Included_l. now apply name_in_fundefs_bound_var_fundefs. 
+          apply Union_Disjoint_r. now eauto with Ensembles_DB.
+          apply Union_Disjoint_r. now eauto with Ensembles_DB.
+          apply Union_Disjoint_r. now eauto with Ensembles_DB.
+          eapply Disjoint_Included_r. now apply Setminus_Included.
+          now eauto with Ensembles_DB.
+        * eapply Disjoint_Included; [| | now apply Hf ].
+          rewrite <- bound_var_Efun.
+          now apply bound_var_occurs_free_Efun_Included.
+          eassumption.
+        * eapply Disjoint_Included_l.
+          eapply Add_functions_LiftedFuns_Included. eassumption.
+          apply Union_Disjoint_l. now eauto with Ensembles_DB.
+          apply Union_Disjoint_r.
+          eapply Disjoint_Included_r. eapply Fundefs_Lambda_lift_free_set_Included.
+          eassumption. now eauto with Ensembles_DB.
+          now eauto with Ensembles_DB.
+        * eapply Disjoint_Included_l.
+          eapply Add_functions_Funs_Included. eassumption.
+          apply Union_Disjoint_l. now eauto with Ensembles_DB.
+          eapply Disjoint_Included_l_sym; [| eassumption ].
+          now apply name_in_fundefs_bound_var_fundefs.
+        * eapply Disjoint_Included_l.
+          eapply Add_functions_FunsFVs_Included_r. eassumption.
+          apply Union_Disjoint_l. now eauto with Ensembles_DB.
+          eapply Disjoint_sym.
+          eapply Disjoint_Included; [ | | now apply HD ].
+          normalize_occurs_free...  now eauto with Ensembles_DB.
+        * eapply Disjoint_Included_r.
+          now eapply occurs_free_Efun_Included.
+          apply Union_Disjoint_r. now eauto with Ensembles_DB.
+          eapply Disjoint_Included_r. now apply name_in_fundefs_bound_var_fundefs.
+          eassumption. 
+        * eapply binding_in_map_antimon;
+          [| eapply binding_in_map_def_funs; eassumption ].
+          apply Union_Included. rewrite Union_assoc.
+          apply Included_Union_preserv_l. normalize_occurs_free. 
+          rewrite Union_assoc, Union_Setminus_Included;
+            now eauto with Ensembles_DB typeclass_instances.
+          eapply Included_trans.
+          eapply Add_functions_FunsFVs_Included_r. eassumption.
+          normalize_occurs_free...
+        * eapply preord_env_P_inj_antimon. eassumption.
+          apply Union_Included.
+          apply Included_Union_preserv_l. normalize_occurs_free. 
+          rewrite Union_commut, Union_assoc, Union_Setminus_Included;
+            now eauto with Ensembles_DB typeclass_instances.
+          now eauto with Ensembles_DB.
     - intros v1 c1 Hleq Hstep. inv Hstep.
       edestruct preord_env_P_inj_getlist_l as [vs' [Hgetl' Hprevs]]; try eassumption.
       normalize_occurs_free...
@@ -2117,12 +1597,55 @@ Section Lambda_lifting_correct.
       eassumption. now eauto. eassumption.
       eapply preord_val_monotonic. eassumption. omega.
     - eapply preord_exp_app_compat.
-      eapply Henv...
+      eapply Henv. now left; eauto.
       eapply Forall2_preord_var_env_map. eassumption.
       normalize_occurs_free...
-    - admit.      
-    - admit.
-  Abort.
+    - inv Hun. eapply preord_exp_prim_compat.
+      + eapply Forall2_preord_var_env_map. eassumption.
+        normalize_occurs_free...
+      + intros vs1 vs2 Hall. eapply IHe; [ eassumption | | | | | | | | | | eassumption ].
+        * eapply Disjoint_Included_l. now eapply image_extend_Included'.
+          eapply Union_Disjoint_l.
+          rewrite occurs_free_Eprim in Him.
+          eapply Disjoint_Included; [ | | now apply Him ].
+          normalize_bound_var...
+          apply image_monotonic. rewrite Setminus_Union_distr...
+          eapply Union_Disjoint_r.
+          eapply Disjoint_Included_l_sym; [| eassumption ]...
+          eapply Disjoint_Singleton_l. intros Hc. inv Hc. now eauto.
+          eapply Hlf. now constructor; eauto.
+        * eapply Disjoint_Included_r; [| eassumption ].
+          now apply bound_var_occurs_free_Eprim_Included.
+        * repeat normalize_bound_var_in_ctx...
+        * repeat normalize_bound_var_in_ctx...
+        * repeat normalize_bound_var_in_ctx...
+        * eapply Disjoint_Included_r. now apply occurs_free_Eprim_Included.
+          eapply Union_Disjoint_r.
+          eapply Disjoint_Included_l ; [| now apply HD].
+          normalize_bound_var... now apply Disjoint_Singleton_r.
+        * eapply binding_in_map_antimon; [| eapply binding_in_map_set; eassumption ]. 
+          apply Union_Included; [| now eauto with Ensembles_DB ].
+          rewrite Union_commut, Union_assoc.
+          apply Included_Union_preserv_l.
+          normalize_occurs_free. rewrite Union_assoc.
+          rewrite Union_Setminus_Included;
+            now eauto with Ensembles_DB typeclass_instances.
+        * eapply preord_env_P_inj_set_alt. 
+          eapply preord_env_P_inj_antimon. eassumption.
+          rewrite Setminus_Union_distr; normalize_occurs_free...
+          eassumption.
+          intros Hc. eapply Him. constructor; eauto.
+          eapply image_monotonic; [| eassumption ].
+          rewrite Setminus_Union_distr; normalize_occurs_free...
+        * eapply Funs_inv_set.
+          intros Hc. eapply Hfun. now constructor; eauto.
+          intros Hc. eapply Hlf. now constructor; eauto.
+          intros Hc. eapply Hfvs. now constructor; eauto.
+          intros Hc. eapply Him. constructor; eauto.
+          eapply image_monotonic; [| eassumption ]...
+          eassumption.
+    - eapply preord_exp_halt_compat.
+      eapply Henv; left; eauto.
+  Qed.
 
-
-  
+End Lambda_lifting_correct.
